reflex/coq/PruneFacts.v
@@ -1,12 +1,15 @@
 Require Import Reflex.
 Require Import ReflexBase.
 Require Import ReflexHVec.
+Require Import ReflexVec.
 Require Import ReflexFin.
 Require Import ReflexDenoted.
 Require Import ReflexIO.
 Require Import List.
+Require Import NIExists.
 
 Require Import Coq.Logic.Eqdep.
+Require Import Sumbool.
 
 Section Prune.
 
@@ -17,19 +20,2580 @@ Variable COMPTDEC : forall (x y : COMPT), decide (x = y).
 Variable COMPS    : COMPT -> compd.
 Variable IENVD    : vcdesc COMPT.
 Variable KSTD     : vcdesc COMPT.
-Variable INIT : init_prog PAYD COMPT COMPS KSTD IENVD.
-Variable HANDLERS : handlers PAYD COMPT COMPS KSTD.
 Definition comp := comp COMPT COMPS.
-Definition Reach := Reflex.Reach PAYD COMPT COMPTDEC COMPS KSTD IENVD INIT.
-Definition ValidExchange := ValidExchange PAYD COMPT COMPTDEC COMPS KSTD HANDLERS.
+Definition cmd := Reflex.cmd PAYD COMPT COMPS KSTD.
 Definition KTrace := KTrace PAYD COMPT COMPS.
 Definition KAction := KAction PAYD COMPT COMPS.
 Definition kstate := kstate PAYD COMPT COMPS KSTD.
 Definition ktr := ktr PAYD COMPT COMPS KSTD.
 Definition Nop := Reflex.Nop PAYD COMPT COMPS KSTD.
+Definition Seq := Reflex.Seq PAYD COMPT COMPS KSTD.
+Definition Send := Reflex.Send PAYD COMPT COMPS KSTD.
+Definition StUpd := Reflex.StUpd PAYD COMPT COMPS KSTD.
+Definition Spawn := Reflex.Spawn PAYD COMPT COMPS KSTD.
+Definition Call := Reflex.Call PAYD COMPT COMPS KSTD.
+Definition Ite := Reflex.Ite PAYD COMPT COMPS KSTD.
+Definition hdlr_term := Reflex.hdlr_term PAYD COMPT COMPS KSTD.
+Definition base_term := Reflex.base_term COMPT.
+Definition match_comp := Reflex.match_comp COMPT COMPTDEC COMPS.
+Definition elt_match := Reflex.elt_match COMPT COMPS.
 
-Require Import NIExists.
-Require Import Ynot.
+Definition locals_eq (envd:vcdesc COMPT)
+  (env1 env2 : sdenote_vcdesc COMPT COMPS envd)
+  (lblr : fin (projT1 envd) -> bool) :=  
+  shvec_erase _ lblr _ env1 = shvec_erase _ lblr _ env2.
+
+Definition ve_st c m envd cmd i s :=
+    hdlr_state_run_cmd PAYD COMPT COMPTDEC COMPS KSTD c m
+    envd s cmd i.
+
+Definition base_term_ok_high envd d (t:base_term envd d) llblr :=
+  match t with
+  | SLit _ => true
+  | NLit _ => true
+  | Var i  => llblr i
+  | _      => false
+  end.
+
+Fixpoint hdlr_term_ok_high ct mt envd c (t:hdlr_term ct mt envd c) vlblr llblr :=
+  match t with
+  | Base _ b    => base_term_ok_high _ _ b llblr
+  | MVar _      => true
+  | StVar i     => vlblr i
+  | CComp       => true
+  | CConf _ _ t => hdlr_term_ok_high _ _ _ _ t vlblr llblr
+  end.
+
+Fixpoint hdlr_expr_ok_high ct mt envd c
+  (e:expr COMPT (hdlr_term ct mt) envd c) vlblr llblr :=
+  match e with
+  | Term _ t => hdlr_term_ok_high _ _ _ _ t vlblr llblr
+  | UnOp _ _ _ e' => hdlr_expr_ok_high _ _ _ _ e' vlblr llblr
+  | BinOp _ _ _ _ e1 e2 => andb (hdlr_expr_ok_high _ _ _ _ e1 vlblr llblr)
+    (hdlr_expr_ok_high _ _ _ _ e2 vlblr llblr)
+  end.
+
+Definition expr_list_ok_high ct mt envd c
+  (es:list (expr COMPT (hdlr_term ct mt) envd c)) vlblr llblr :=
+  fold_right (fun e => andb
+    (hdlr_expr_ok_high ct mt envd c e vlblr llblr)) true es.
+
+Fixpoint pl_expr_ok_high ct mt envd n vd
+  (ple:payload_expr' COMPT (hdlr_term ct mt) envd n vd) vlblr llblr :=
+  match n as _n return
+    forall (_vd:vdesc' _n) (ple:payload_expr' COMPT (hdlr_term ct mt) envd _n _vd), _
+  with
+  | O => fun _ _ => true
+  | S n' => fun vd =>
+    match vd as _vd return
+      payload_expr' COMPT (hdlr_term ct mt) envd (S n') _vd -> _
+    with
+    | (vd0, vd') =>
+      fun ple =>
+        andb (hdlr_expr_ok_high ct mt envd _ (fst ple) vlblr llblr)
+          (pl_expr_ok_high ct mt envd n' _ (snd ple) vlblr llblr)
+    end
+  end vd ple.
+
+Fixpoint get_writes envd term (cmd:cmd term envd) :=
+  match cmd in Reflex.cmd _ _ _ _ _ _envd return
+    fin (projT1 _envd) -> bool
+  with
+  | Reflex.Seq _ cmd1 cmd2 =>
+    fun i => andb (get_writes _ _ cmd1 i)
+      (get_writes _ _ cmd2 i)
+  | Reflex.Ite _ _ cmd1 cmd2 =>
+    fun i => andb (get_writes _ _ cmd1 i)
+      (get_writes _ _ cmd2 i)
+  | Reflex.Spawn _ _ _ i' _ =>
+    fun i => if fin_eq_dec i i' then false else true
+  | Reflex.Call _ _ _ i' _ =>
+    fun i => if fin_eq_dec i i' then false else true
+  | Reflex.CompLkup _ _ cmd1 cmd2 =>
+    fun i => andb (get_writes _ _ cmd1 (lift_fin i))
+      (get_writes _ _ cmd2 i)
+  | _ =>
+    fun _ => true
+  end.
+
+Definition cp_incl cp1 cp2 :=
+  forall c, implb (match_comp cp1 c)
+    (match_comp cp2 c) = true.
+
+Definition elt_incl d oelt1 oelt2 :=
+  forall elt,
+    implb (elt_match d elt oelt1)
+    (elt_match d elt oelt2) = true.
+
+Lemma desc_2 : forall (d:desc),
+  ex (fun s1:s[[d]] => ex (fun s2:s[[d]] => s1 <> s2)).
+Proof.
+  destruct d.
+    exists FALSE. exists TRUE. discriminate.
+    Local Transparent str_of_string.
+    exists (str_of_string ""). exists (str_of_string "a").
+    discriminate.
+    exists FALSE. exists TRUE. discriminate.
+Qed.
+
+Lemma desc_neq : forall (d:desc) (s:s[[d]]),
+  exists s', s <> s'.
+Proof.
+  intros d s. pose proof (desc_2 d).
+  destruct H. destruct H.
+  destruct d.
+    destruct (num_eq s x).
+      exists x0. congruence.
+      exists x. auto.
+
+    destruct (str_eq s x).
+      exists x0. congruence.
+      exists x. auto.
+
+    destruct (fd_eq s x).
+      exists x0. congruence.
+      exists x. auto.
+Qed.
+
+Lemma elt_incl_iff : forall d oelt1 oelt2,
+  elt_incl d oelt1 oelt2 <->
+  oelt2 = None \/ oelt1 = oelt2.
+Proof.
+  intros d oelt1 oelt2.
+  split.
+    intro Hincl. destruct oelt2.
+      right. unfold elt_incl, elt_match in Hincl. simpl in Hincl.
+      destruct oelt1.
+        destruct d; specialize (Hincl s0); simpl in *;
+          repeat match goal with
+                 | [ _ : context[ if ?e then _ else _ ] |- _ ]
+                   => destruct e
+                 end; try solve [subst s; auto | discriminate |
+                   specialize (n (Logic.eq_refl _)); contradiction].
+
+        pose proof (desc_neq d s). destruct H.
+        specialize (Hincl x). destruct d;
+        match goal with
+        | [ _ : context[ if ?e then _ else _ ] |- _ ]
+          => destruct e
+        end; try discriminate; try contradiction.
+
+      left. auto.
+
+    intro H. destruct H.
+      subst oelt2. unfold elt_incl. simpl.
+      intros. unfold implb. destruct (elt_match d elt oelt1); auto.
+
+      subst oelt1. unfold elt_incl. simpl. intros.
+      unfold implb. destruct (elt_match d elt oelt2); auto.
+Qed.
+
+Definition elt_incl_dec d oelt1 oelt2 :
+  decide (elt_incl d oelt1 oelt2).
+Proof.
+  destruct oelt2.
+    destruct oelt1.
+    destruct d.
+      destruct (num_eq s0 s);
+        [left; subst s; apply elt_incl_iff; auto
+          | right; intro H; apply elt_incl_iff in H;
+            destruct H; try inversion H; contradiction].
+      destruct (str_eq s0 s);
+        [left; subst s; apply elt_incl_iff; auto
+          | right; intro H; apply elt_incl_iff in H;
+            destruct H; try inversion H; contradiction].
+      destruct (fd_eq s0 s);
+        [left; subst s; apply elt_incl_iff; auto
+          | right; intro H; apply elt_incl_iff in H;
+            destruct H; try inversion H; contradiction].
+
+    right. intro H. apply elt_incl_iff in H. destruct H; discriminate.
+
+    left. apply elt_incl_iff. auto.
+Qed.
+
+Definition default_desc (d:desc) : s[[d]] :=
+match d with
+| num_d => FALSE
+| str_d => nil
+| fd_d => devnull
+end.
+
+Definition default_desc_match (d:desc) (oelt:sdenote_desc_conc_pat d)
+  : s[[d]] :=
+match oelt with
+| Some e => e
+| None => default_desc d
+end.
+
+Lemma default_desc_match_ok : forall d oelt,
+  elt_match d (default_desc_match d oelt) oelt = true.
+Proof.
+  intros d oelt.
+  destruct oelt; auto.
+  simpl. destruct d;
+  match goal with
+  |- context [ if ?e then _ else _ ]
+    => destruct e
+  end; auto.
+Qed.
+
+Definition non_match_vdesc n (vd:svec desc n) vdp :
+  sig (fun v:s[[vd]] => shvec_match vd sdenote_desc sdenote_desc_conc_pat elt_match v vdp = true).
+Proof.
+  induction n.
+    exact (exist _ tt (Logic.eq_refl _)).
+
+    destruct vd as [d vd']. destruct vdp as [od vdp']. simpl in *.
+    specialize (IHn vd' vdp'). destruct IHn.
+    refine (exist _ (default_desc_match d od, x) _).
+    rewrite default_desc_match_ok; auto.
+Qed.
+
+Definition cfgp_incl (cfgd:vdesc) cfgp1 cfgp2 :=
+  forall cfg, implb 
+    (shvec_match (projT2 cfgd)
+      sdenote_desc sdenote_desc_conc_pat elt_match
+      cfg cfgp1)
+    (shvec_match (projT2 cfgd)
+      sdenote_desc sdenote_desc_conc_pat elt_match
+      cfg cfgp2) = true.
+
+Definition cfgp_incl_dec (cfgd:vdesc) cfgp1 cfgp2 :
+  decide (cfgp_incl cfgd cfgp1 cfgp2).
+Proof.
+  destruct cfgd as [n cfgd]. unfold cfgp_incl.
+  induction n.
+    auto.
+
+    simpl in *. destruct cfgd as [? cfgd'].
+    destruct cfgp1 as [oelt1 cfgp1']. destruct cfgp2 as [oelt2 cfgp2'].
+    specialize (IHn cfgd' cfgp1' cfgp2').
+    destruct (elt_incl_dec d oelt1 oelt2).
+      destruct IHn.
+        left. intro cfg. destruct cfg as [elt cfg'].
+        specialize (e elt).
+        destruct (elt_match d elt oelt1).
+          destruct (elt_match d elt oelt2); try discriminate.
+          simpl. auto.
+          
+          auto.
+
+        right. intro.
+
+contradict n0. intro cfg.
+specialize (H (default_desc_match d oelt1, cfg)).
+specialize (e (default_desc_match d oelt1)). simpl in *.
+rewrite default_desc_match_ok in *. simpl in *.
+rewrite e in *. simpl in *. auto.
+
+right. intro. contradict n0.
+unfold elt_incl. intro elt.
+
+pose proof (non_match_vdesc n cfgd' cfgp1') as rest.
+destruct rest as [rest Hrest].
+specialize (H (elt, rest)). simpl in *. rewrite Hrest in H.
+simpl in *. destruct (elt_match d elt oelt1); auto.
+simpl in *. destruct (elt_match d elt oelt2); auto.
+Defined.
+
+Definition cp_incl_dec cp1 cp2 : decide (cp_incl cp1 cp2).
+Proof.
+  destruct cp1 as [ct1 cfg1]; destruct cp2 as [ct2 cfg2].
+  destruct (COMPTDEC ct1 ct2).
+    subst ct1. 
+    destruct (cfgp_incl_dec _ cfg1 cfg2).
+      left. unfold cp_incl, match_comp, Reflex.match_comp, match_comp_pf.
+      simpl. intro cp.
+      destruct (COMPTDEC (comp_type COMPT COMPS cp) ct2); auto. destruct e.
+      specialize (c (comp_conf _ _ cp)). unfold elt_match in *.
+      destruct (shvec_match
+              (projT2 (comp_conf_desc COMPT COMPS (comp_type COMPT COMPS cp)))
+              sdenote_desc sdenote_desc_conc_pat (Reflex.elt_match COMPT COMPS)
+              (comp_conf COMPT COMPS cp) cfg1);
+      destruct (shvec_match
+              (projT2 (comp_conf_desc COMPT COMPS (comp_type COMPT COMPS cp)))
+              sdenote_desc sdenote_desc_conc_pat (Reflex.elt_match COMPT COMPS)
+              (comp_conf COMPT COMPS cp) cfg2); auto.
+
+      right. intro. contradict n. intro cfg. unfold cp_incl in *.
+      specialize (H {|comp_type:=ct2; comp_fd:=devnull; comp_conf:=cfg|}).
+      unfold match_comp, Reflex.match_comp, match_comp_pf in *. simpl in *.
+      destruct (COMPTDEC ct2 ct2); auto.
+      rewrite UIP_refl with (p:=e) in *. unfold elt_match in *.
+      destruct (shvec_match (projT2 (comp_conf_desc COMPT COMPS ct2))
+                 sdenote_desc sdenote_desc_conc_pat
+                 (Reflex.elt_match COMPT COMPS) cfg cfg1);
+      destruct (shvec_match (projT2 (comp_conf_desc COMPT COMPS ct2))
+                 sdenote_desc sdenote_desc_conc_pat
+                 (Reflex.elt_match COMPT COMPS) cfg cfg2); auto.
+
+      right. intro.
+      pose proof (non_match_vdesc _ _ cfg1) as Hmatch.
+      destruct Hmatch as [v Hv].
+      specialize (H {|comp_type:=ct1;
+        comp_fd:=devnull;
+        comp_conf:=v|}).
+      unfold match_comp, Reflex.match_comp, match_comp_pf in *.
+      simpl in *. destruct (COMPTDEC ct1 ct2); try contradiction.
+      destruct (COMPTDEC ct1 ct1).
+      rewrite UIP_refl with (p:=e) in *. unfold elt_match in *.
+      rewrite Hv in *. discriminate.
+      contradict n1. auto.
+Qed.
+
+(*Definition high_cp_dec cp clblr :
+  decide (high_comp_pat COMPT COMPTDEC COMPS cp
+    (lblr_match_comp COMPT COMPTDEC COMPS clblr)).
+Proof.
+  induction clblr.
+    left. unfold high_comp_pat. intros. simpl. auto.
+
+    destruct IHclblr.
+      left. unfold high_comp_pat. intros c Hmatch.
+      specialize (h c Hmatch). unfold lblr_match_comp in *.
+      destruct clblr. simpl in *. auto. simpl in *.
+      rewrite h. auto.
+
+      destruct (cp_incl_dec cp a).
+        left. unfold high_comp_pat. intros comp Hmatch.
+        specialize (c comp). unfold match_comp, NIExists.match_comp in *. rewrite Hmatch in c.
+        simpl in *. unfold NIExists.match_comp. rewrite c. rewrite Bool.orb_true_r. auto.
+
+        right. intro. unfold high_comp_pat in *.
+      admit.
+Qed.*)
+
+Fixpoint get_llblr ct mt envd cmd vlblr llblr :=
+  match cmd in Reflex.cmd _ _ _ _ _ _envd return
+    (fin (projT1 _envd) -> bool) -> _
+  with
+  | Reflex.Seq _ cmd1 cmd2 => fun llblr =>
+    let llblr1 := get_llblr ct mt _ cmd1 vlblr llblr in
+    get_llblr ct mt _ cmd2 vlblr llblr1
+  | Reflex.Ite envd e cmd1 cmd2 => fun llblr =>
+    if hdlr_expr_ok_high ct mt envd _ e vlblr llblr
+    then fun i => andb (get_llblr ct mt _ cmd1 vlblr llblr i)
+      (get_llblr ct mt _ cmd2 vlblr llblr i)
+    else fun i => andb (get_writes _ _ cmd1 i) (get_writes _ _ cmd2 i)
+  | Reflex.CompLkup _ _ cmd1 cmd2 => fun _ =>
+    fun i => andb (get_writes _ _ cmd1 (lift_fin i)) (get_writes _ _ cmd2 i)
+  | Reflex.Spawn _ t e i _ => fun llblr =>
+    if pl_expr_ok_high ct mt _ _ _ e vlblr llblr
+    then fun i' =>
+      if fin_eq_dec i i'
+      then true
+      else llblr i'
+    else fun i' =>
+      if fin_eq_dec i i'
+      then false
+      else llblr i'
+  | _       => fun llblr => llblr
+  end llblr.
+
+(*Fixpoint get_candidate_pats clblr ct :
+  list (shvec sdenote_desc_conc_pat (projT2 (compd_conf (COMPS ct)))) :=
+  match clblr with
+  | nil => nil
+  | a::clblr' => 
+    match COMPTDEC ct (conc_pat_type _ COMPS a) with
+    | left EQ =>
+      match EQ in _ = _ct return
+        shvec sdenote_desc_conc_pat (projT2 (compd_conf (COMPS _ct))) -> _
+      with
+      | Logic.eq_refl => fun cfg0 =>
+        cfg0::get_candidate_pats clblr' ct
+      end (conc_pat_conf _ COMPS a)
+    | right _ => get_candidate_pats clblr' ct
+    end
+  end.
+
+Definition desc_val_eq {d:desc}
+  : forall (e1 e2:s[[d]]), decide (e1 = e2) :=
+  match d with
+  | num_d => num_eq
+  | str_d => str_eq
+  | fd_d  => fd_eq
+  end.
+
+Definition merge_desc_pats (d:desc) (o1 o2:option s[[d]])
+  : option s[[d]] :=
+  match o1 with
+  | Some e1 =>
+    match o2 with
+    | Some e2 => if desc_val_eq e1 e2
+                 then Some e1
+                 else None
+    | None    => None
+    end
+  | None    => None
+  end.
+
+Fixpoint merge_cfgps n :
+  forall (vd:svec desc n), shvec sdenote_desc_conc_pat vd ->
+      shvec sdenote_desc_conc_pat vd -> shvec sdenote_desc_conc_pat vd :=
+  match n as _n return
+    forall (vd:svec desc _n), shvec sdenote_desc_conc_pat vd ->
+      shvec sdenote_desc_conc_pat vd -> shvec sdenote_desc_conc_pat vd
+  with
+  | O => fun _ _ _ => tt
+  | S n' => fun vd =>
+    match vd as _vd return
+      shvec (n:=S n') sdenote_desc_conc_pat _vd ->
+      shvec (n:=S n') sdenote_desc_conc_pat _vd ->
+      shvec (n:=S n') sdenote_desc_conc_pat _vd
+    with
+    | (vd0, vd') => fun cfgp1 cfgp2 =>
+      (merge_desc_pats vd0 (fst cfgp1) (fst cfgp2), merge_cfgps n' vd' (snd cfgp1) (snd cfgp2))
+    end
+  end.
+
+Definition merge_all_cfgps ct cfgps cfgp0 :=
+  fold_right (merge_cfgps _ (projT2 (compd_conf (COMPS ct))))
+  cfgp0 cfgps.
+*)
+(*Definition get_ccomp_vals ct cfgps cfgp0 :=
+  {| conc_pat_type:=ct
+   ; conc_pat_conf:=fold_right
+       (merge_cfgps _ (projT2 (compd_conf (COMPS ct))))
+       cfgp0 cfgps |}.*)
+
+Lemma compcd_inj : forall ct ct',
+  Comp COMPT ct = Comp COMPT ct' ->
+  ct = ct'.
+Proof.
+  intros. injection H. auto.
+Qed.
+
+Definition peval_hdlr_term {cd envd} ct mt (t : hdlr_term ct mt envd cd)
+  (v:shvec sdenote_desc_conc_pat (projT2 (compd_conf (COMPS ct))))
+  : option (sdenote_cdesc COMPT COMPS cd).
+  destruct t.
+    exact None.
+    exact None.
+refine (
+  match t in Reflex.hdlr_term _ _ _ _ _ _ _ _c return
+      _c = Comp COMPT ct' -> _
+  with
+  | CComp => fun EQ =>
+    match compcd_inj _ _ EQ in _ = _ct return
+      forall (i:fin (projT1 (comp_conf_desc COMPT COMPS _ct))),
+      option
+      (sdenote_cdesc COMPT COMPS
+       (Desc COMPT (svec_ith (projT2 (comp_conf_desc COMPT COMPS _ct)) i)))
+    with
+    | Logic.eq_refl => fun i =>
+      shvec_ith _ _ v i
+    end i
+  | _ => fun _ => None
+  end (Logic.eq_refl _)).
+      exact None.
+    exact None.
+Defined.
+
+Lemma peval_hdlr_term_sound : forall cd envd ct mt
+  (t:hdlr_term ct mt envd cd) cfgp v cfg f pl,
+  peval_hdlr_term ct mt t cfgp = Some v ->
+  (forall i v,
+    shvec_ith sdenote_desc_conc_pat (projT2 (compd_conf (COMPS ct))) cfgp i =
+    Some v ->
+    shvec_ith sdenote_desc (projT2 (compd_conf (COMPS ct))) cfg i = v) ->
+  (forall st env,
+    eval_hdlr_term PAYD COMPT COMPS KSTD
+    (Build_comp COMPT COMPS ct f cfg)
+    (Build_msg PAYD mt pl) st t env = v).
+Proof.
+  intros cd envd ct mt t cfgp v cfg f pl Hpeval Hcfgp st env. Require Import Program.
+  generalize dependent v. dependent inversion t; try discriminate.
+  dependent destruction h; try discriminate. admit.
+  generalize dependent h0. (* rewrite <- x.
+  rewrite <- x0. generalize (Comp COMPT ct').
+
+revert x0. generalize (svec_ith (projT2 KSTD) i0).
+  intros c Heqc. dependent rewrite <- Heqc in h0.
+  dependent rewrite <- x0 in h0.
+  generalize dependent i.
+  simpl.
+
+dependent inversion h with (fun (hndx : cdesc COMPT)
+(hterm : Reflex.hdlr_term PAYD COMPT COMPS KSTD ct mt envd hndx) =>
+
+match hndx as _hndx return
+  sdenote_cdesc COMPT COMPS _hndx ->
+  Prop
+with
+| Comp ct1 => fun x =>
+
+forall (i : fin (projT1 (comp_conf_desc COMPT COMPS ct1)))
+     (v : sdenote_desc (svec_ith (projT2 (comp_conf_desc COMPT COMPS ct1)) i)),
+   match
+     h in (Reflex.hdlr_term _ _ _ _ _ _ _ _c)
+     return
+       (_c = Comp COMPT ct' ->
+        option
+          (sdenote_desc
+             (svec_ith (projT2 (comp_conf_desc COMPT COMPS ct1)) i)))
+   with
+   | Base d _ => fun _ : d = Comp COMPT ct' => None
+   | CComp =>
+       fun EQ : Comp COMPT ct = Comp COMPT ct' =>
+       match
+         compcd_inj ct ct' EQ in (_ = _ct)
+         return
+           (forall i0 : fin (projT1 (comp_conf_desc COMPT COMPS _ct)),
+            option
+              (sdenote_desc
+                 (svec_ith (projT2 (comp_conf_desc COMPT COMPS _ct)) i0)))
+       with
+       | eq_refl =>
+           fun i0 : fin (projT1 (comp_conf_desc COMPT COMPS ct)) =>
+           shvec_ith sdenote_desc_conc_pat (projT2 (compd_conf (COMPS ct)))
+             cfgp i0
+       end i
+   | CConf ct'0 i0 _ =>
+       fun
+         _ : Desc COMPT
+               (svec_ith (projT2 (comp_conf_desc COMPT COMPS ct'0)) i0) =
+             Comp COMPT ct' => None
+   | MVar i0 =>
+       fun
+         _ : Desc COMPT (svec_ith (projT2 (lkup_tag PAYD mt)) i0) =
+             Comp COMPT ct' => None
+   | StVar i0 => fun _ : svec_ith (projT2 KSTD) i0 = Comp COMPT ct' => None
+   end (eq_refl (Comp COMPT ct')) = Some v ->
+   match
+     projT2
+       x in (_ = _ct)
+     return
+       (forall _i : fin (projT1 (comp_conf_desc COMPT COMPS _ct)),
+        sdenote_desc (svec_ith (projT2 (comp_conf_desc COMPT COMPS _ct)) _i))
+   with
+   | eq_refl =>
+       fun
+         i0 : fin
+                (projT1
+                   (comp_conf_desc COMPT COMPS
+                      (comp_type COMPT COMPS
+                         (projT1
+                            x)))) =>
+       shvec_ith sdenote_desc
+         (projT2
+            (comp_conf_desc COMPT COMPS
+               (comp_type COMPT COMPS
+                  (projT1
+                     x))))
+         (comp_conf COMPT COMPS
+            (projT1
+               x)) i0
+   end i = v
+
+| _ => fun _ => True
+end
+
+(eval_hdlr_term PAYD COMPT COMPS KSTD
+                  {| comp_type := ct; comp_fd := f; comp_conf := cfg |}
+                  {| tag := mt; pay := pl |} st h env)
+
+).
+
+
+
+
+
+
+
+
+
+
+
+
+
+
+
+
+
+
+
+
+
+
+
+
+
+
+
+
+
+
+
+
+
+
+
+
+
+
+
+
+
+
+
+
+
+
+
+
+
+
+
+
+
+
+
+
+
+
+
+
+
+
+
+
+
+
+
+
+
+
+
+
+
+
+
+
+
+forall i : fin (projT1 (comp_conf_desc COMPT COMPS ct1)),
+   Desc COMPT (svec_ith (projT2 (comp_conf_desc COMPT COMPS ct1)) i) = cd ->
+   forall
+     v : sdenote_cdesc COMPT COMPS
+           (Desc COMPT (svec_ith (projT2 (comp_conf_desc COMPT COMPS ct1)) i)),
+   y = Some v ->
+match
+     projT2 x in (_ = _ct)
+     return
+       (forall _i : fin (projT1 (comp_conf_desc COMPT COMPS _ct)),
+        sdenote_desc (svec_ith (projT2 (comp_conf_desc COMPT COMPS _ct)) _i))
+   with
+   | eq_refl =>
+       fun
+         i0 : fin
+                (projT1
+                   (comp_conf_desc COMPT COMPS
+                      (comp_type COMPT COMPS
+                         (projT1 x)))) =>
+       shvec_ith sdenote_desc
+         (projT2
+            (comp_conf_desc COMPT COMPS
+               (comp_type COMPT COMPS
+                  (projT1 x))))
+         (comp_conf COMPT COMPS
+            (projT1 x)) i0
+   end i = v
+
+| _ => fun _ => True
+end
+
+(eval_hdlr_term PAYD COMPT COMPS KSTD
+                  {| comp_type := ct; comp_fd := f; comp_conf := cfg |}
+                  {| tag := mt; pay := pl |} st hterm env)
+
+). simpl. discriminate. simpl. admit. simpl. generalize (shvec_ith (sdenote_cdesc COMPT COMPS) (projT2 KSTD) st i). generalize (svec_ith (projT2 KSTD) i).
+
+  unfold eval_hdlr_term. simpl.
+  simpl. Require Import Program. simpl. dependent destruction h; try discriminate. admit. dependent inversion h. unfold eval_hdlr_term; simpl
+  intros v. 
+  rewrite UIP_refl with (p:=compcd_inj ct' ct' eq_refl). intro Hpeval. simpl in *. auto.
+(*apply JMeq_eq_dep in x; auto. apply eq_dep_eq_sigT in x. SearchAbout existT.
+   inversion x.*)*)
+  admit.
+Qed.
+
+Definition peval_expr {cd envd} ct mt
+  (e:expr COMPT (hdlr_term ct mt) envd cd)
+  (v:shvec sdenote_desc_conc_pat (projT2 (compd_conf (COMPS ct))))
+  : option (sdenote_cdesc COMPT COMPS cd).
+induction e.
+  exact (peval_hdlr_term ct mt t v).
+  
+  destruct IHe.
+    exact (Some (eval_unop COMPT COMPS _ _ u s)).
+    exact None.
+
+  destruct IHe1.
+    destruct IHe2.
+      exact (Some (eval_binop COMPT COMPS _ _ _ b s s0)).
+      exact None.
+
+    exact None.
+Defined.
+
+Lemma peval_expr_sound : forall cd envd ct mt
+  (e:expr COMPT (hdlr_term ct mt) envd cd) cfgp v cfg f pl,
+  peval_expr ct mt e cfgp = Some v ->
+  (forall i v,
+    shvec_ith sdenote_desc_conc_pat (projT2 (compd_conf (COMPS ct))) cfgp i =
+    Some v ->
+    shvec_ith sdenote_desc (projT2 (compd_conf (COMPS ct))) cfg i = v) ->
+  (forall st env,
+    eval_hdlr_expr PAYD COMPT COMPS KSTD
+    (Build_comp COMPT COMPS ct f cfg)
+    (Build_msg PAYD mt pl) st env e = v).
+Proof.
+  intros cd envd ct mt e cfgp v cfg f pl Hpeval Hcfgp st env.
+
+  induction e; simpl in *.
+    eapply peval_hdlr_term_sound with (v:=v); eauto.
+    
+    destruct (peval_expr ct mt e cfgp); try discriminate.
+    inversion Hpeval. rewrite IHe with (v:=s); auto.
+
+    destruct (peval_expr ct mt e1 cfgp); try discriminate;
+    destruct (peval_expr ct mt e2 cfgp); try discriminate.
+    inversion Hpeval. rewrite IHe1 with (v:=s); auto;
+    rewrite IHe2 with (v:=s0); auto.
+Qed.
+
+Definition peval_oexpr {cd envd} ct mt
+  (oe:option (expr COMPT (hdlr_term ct mt) envd cd))
+  (v:shvec sdenote_desc_conc_pat (projT2 (compd_conf (COMPS ct))))
+  : option (sdenote_cdesc COMPT COMPS cd).
+destruct oe.
+  exact (peval_expr ct mt e v).
+  exact None.
+Defined.
+
+Lemma peval_oexpr_sound : forall cd envd ct mt
+  (oe:option (expr COMPT (hdlr_term ct mt) envd cd)) cfgp v cfg f pl,
+  peval_oexpr ct mt oe cfgp = Some v ->
+  (forall i v,
+    shvec_ith sdenote_desc_conc_pat (projT2 (compd_conf (COMPS ct))) cfgp i =
+    Some v ->
+    shvec_ith sdenote_desc (projT2 (compd_conf (COMPS ct))) cfg i = v) ->
+  (forall st env,
+    eval_oexpr COMPT COMPS (hdlr_term ct mt)
+    (fun d envd env t =>
+      eval_hdlr_term PAYD COMPT COMPS KSTD
+      (Build_comp COMPT COMPS ct f cfg)
+      (Build_msg PAYD mt pl) st t env) env oe = Some v).
+Proof.
+  intros cd envd ct mt oe cfgp v cfg f pl Hpeval Hcfgp st env.
+  destruct oe; try discriminate.
+    simpl in *. f_equal.
+    pose proof (peval_expr_sound cd envd ct mt e cfgp v cfg f pl Hpeval Hcfgp st env).
+    unfold eval_hdlr_expr in *. auto.
+Qed.
+
+Fixpoint peval_payload_oexpr ct mt envd n : forall (vd:svec desc n),
+  payload_oexpr' COMPT (hdlr_term ct mt) envd n vd ->
+  shvec sdenote_desc_conc_pat (projT2 (compd_conf (COMPS ct))) ->
+  shvec sdenote_desc_conc_pat vd.
+intros vd cfgpe cfgp.
+induction n.
+  exact tt.
+
+  simpl in *. destruct vd as [vd0 vd']. destruct cfgpe as [oe cfgpe'].
+  exact (peval_oexpr ct mt oe cfgp, peval_payload_oexpr ct mt envd n vd' cfgpe' cfgp).
+Defined.
+
+Lemma peval_payload_oexpr_sound : forall envd ct mt n vd
+  (cfgpe:payload_oexpr' COMPT (hdlr_term ct mt) envd n vd) cfgp cfg f pl,
+  (forall i v,
+    shvec_ith sdenote_desc_conc_pat (projT2 (compd_conf (COMPS ct))) cfgp i =
+    Some v ->
+    shvec_ith sdenote_desc (projT2 (compd_conf (COMPS ct))) cfg i = v) ->
+  (forall st env,
+    cfgp_incl _
+     (eval_hdlr_payload_oexpr PAYD COMPT COMPS KSTD
+       (Build_comp COMPT COMPS ct f cfg)
+       (Build_msg PAYD mt pl) st envd env (existT _ n vd) cfgpe)
+     (peval_payload_oexpr ct mt envd n vd cfgpe cfgp)).
+Proof.
+  intros envd ct mt n vd cfgpe cfgp cfg f pl Hcfgp st env cfg'.
+  apply Bool.leb_implb. unfold Bool.leb.
+  match goal with
+  |- if ?e then _ else _ =>
+    destruct e as [? | ?]_eqn; auto
+  end.
+  induction n.
+    auto.
+
+    destruct vd. destruct cfgpe. destruct cfg'. simpl in *.
+    apply andb_prop in Heqb. destruct Heqb.
+    destruct (peval_oexpr ct mt o cfgp) as [? | ?]_eqn.
+      rewrite peval_oexpr_sound with (v:=s2) (cfgp:=cfgp) in H; auto.
+      rewrite H. simpl. apply IHn; auto.
+
+      simpl. apply IHn; auto.
+Qed.
+
+Definition is_high_comp_pat ct mt envd cp clblr : bool :=
+  let conf := peval_payload_oexpr ct _ _ _ _
+    (comp_pat_conf COMPT COMPS (hdlr_term ct mt) envd cp) 
+    (clblr ct) in
+  let cpt := comp_pat_type _ _ _ _ cp in
+  (projT1 (bool_of_sumbool (cp_incl_dec (Build_conc_pat COMPT COMPS cpt conf)
+    (Build_conc_pat COMPT COMPS cpt (clblr cpt))))).
+
+(*  match get_candidate_pats clblr ct with
+  | cfg0::cfgs' =>
+    let merged := merge_all_cfgps ct cfgs' cfg0 in
+    let conf := get_conc_pat_conf ct _ _ _ _ (comp_pat_conf COMPT COMPS (hdlr_term ct mt) envd cp) merged in
+    existsb (fun cp' =>
+      (proj1_sig (bool_of_sumbool
+      (cp_incl_dec
+        (Build_conc_pat COMPT COMPS
+          (comp_pat_type _ _ _ _ cp) conf) cp')))) clblr
+  | nil => false
+  end.*)
+
+Lemma is_high_comp_pat_sound : forall c m envd cp clblr,
+  lblr_match_comp COMPT COMPTDEC COMPS clblr c = true ->
+  is_high_comp_pat (comp_type _ _ c) (tag _ m) envd cp clblr = true ->
+  forall st env,
+    high_comp_pat COMPT COMPTDEC COMPS
+      (eval_hdlr_comp_pat PAYD COMPT COMPS KSTD c m st envd env cp)
+      (lblr_match_comp COMPT COMPTDEC COMPS clblr).
+Proof.
+  intros c m envd cp clblr Hmatch Hhigh st env.
+  unfold is_high_comp_pat in Hhigh.
+  destruct cp as [cpt cpfg]. destruct c as [ct f cfg].
+  destruct m as [mt pl]. simpl in *.
+  unfold high_comp_pat. intros c' Hmatch'.
+  match goal with
+  | [ _ : context [ cp_incl_dec ?cp1 ?cp2 ] |- _ ]
+    => destruct (cp_incl_dec cp1 cp2); try discriminate
+  end. unfold cp_incl in *. clear Hhigh. specialize (c c').
+  unfold match_comp, NIExists.match_comp, Reflex.match_comp, match_comp_pf in *.
+  simpl in *. unfold hdlr_term, CT, CTAG in *.
+  destruct (COMPTDEC (comp_type COMPT COMPS c') cpt); try discriminate.
+  destruct e.
+  pose proof (peval_payload_oexpr_sound envd ct mt _ _ cpfg (clblr ct) cfg f pl).
+Lemma high_comp_cfgp_sound : forall ct f cfg clblr,
+  lblr_match_comp COMPT COMPTDEC COMPS clblr
+  {| comp_type := ct; comp_fd := f; comp_conf := cfg |} = true ->
+  (forall (i : fin (projT1 (comp_conf_desc COMPT COMPS ct)))
+         (v : s[[svec_ith (projT2 (comp_conf_desc COMPT COMPS ct)) i]]),
+       shvec_ith sdenote_desc_conc_pat (projT2 (comp_conf_desc COMPT COMPS ct))
+         (clblr ct) i = Some v ->
+       shvec_ith sdenote_desc (projT2 (comp_conf_desc COMPT COMPS ct)) cfg i = v).
+Proof.
+  intros ct f cfg clblr Hlblr i v Hith.
+  unfold lblr_match_comp, NIExists.match_comp,
+    Reflex.match_comp, match_comp_pf in Hlblr. simpl in *.
+  destruct (COMPTDEC ct ct); try discriminate.
+  rewrite UIP_refl with (p:=e) in Hlblr.
+Lemma high_comp_cfgp_sound' : forall n vd v (i:fin n) cfg s,
+  shvec_match vd sdenote_desc sdenote_desc_conc_pat
+    (Reflex.elt_match COMPT COMPS) cfg v = true ->
+  shvec_ith sdenote_desc_conc_pat vd v i = Some s ->
+  shvec_ith sdenote_desc vd cfg i = s.
+Proof.
+  intros n vd v i cfg s Hmatch Hith.
+  induction n.
+    contradiction.
+
+    destruct vd as [vd0 vd']. destruct cfg as [cfg0 cfg'].
+    destruct v as [v0 v']. simpl in *.
+    apply andb_prop in Hmatch. destruct Hmatch as [Hmatch_elt ?].
+    destruct i.
+      apply IHn with (v:=v'); auto.
+
+      rewrite Hith in Hmatch_elt. simpl in Hmatch_elt.
+      destruct vd0;
+        match goal with
+        | [ _ : context [ if ?e then _ else _ ] |- _ ]=>
+          destruct e; try discriminate; auto
+        end.
+Qed.
+apply high_comp_cfgp_sound' with (v:=
+  
+pose (
+fun v0 : sigT vdesc' =>
+ forall cfg : sdenote_vdesc v0,
+ (if if shvec_match (projT2 v0) sdenote_desc sdenote_desc_conc_pat
+          (Reflex.elt_match COMPT COMPS) cfg (clblr ct)
+     then Some eq_refl
+     else None
+  then true
+  else false) = true ->
+ forall (i : fin (projT1 v0)) (v : sdenote_desc (svec_ith (projT2 v0) i)),
+ shvec_ith sdenote_desc_conc_pat (projT2 v0) (clblr ct) i = Some v ->
+ shvec_ith sdenote_desc (projT2 v0) cfg i = v).
+  destruct (comp_conf_desc COMPT COMPS ct).
+  cut (shvec_match
+                 (projT2
+                    (comp_conf_desc COMPT COMPS (comp_type COMPT COMPS c')))
+                 sdenote_desc sdenote_desc_conc_pat elt_match
+                 (comp_conf COMPT COMPS c')
+                 (get_conc_pat_conf ct (tag PAYD m) envd
+                    (projT1
+                       (comp_conf_desc COMPT COMPS (comp_type COMPT COMPS c')))
+                    (projT2
+                       (comp_conf_desc COMPT COMPS (comp_type COMPT COMPS c')))
+                    cpfg (clblr ct)) = true).
+    intro H. unfold elt_match in *. rewrite H in *.
+    unfold lblr_match_comp, NIExists.match_comp, Reflex.match_comp, match_comp_pf.
+    simpl in *. destruct (COMPTDEC (comp_type COMPT COMPS c') (comp_type COMPT COMPS c')); try intuition.
+    rewrite UIP_refl with (p:=e). auto.
+
+    clear c. destruct c' as [ct' ? cfg']. simpl in *.
+    destruct (comp_conf_desc COMPT COMPS ct') as [n cfgd].
+    induction n.
+      auto.
+
+      destruct cfgd. destruct cpfg. destruct cfg'. simpl in *.
+      destruct o. simpl in *. 
+dependent inversion e with (
+  fun (c : cdesc COMPT)
+   (e : expr COMPT (Reflex.hdlr_term PAYD COMPT COMPS KSTD ct (tag PAYD m))
+          envd c) =>
+ (let (elt', rest') :=
+      get_conc_pat_conf ct (tag PAYD m) envd (S n) 
+        (d, s) (Some e, p) (clblr ct) in
+  (elt_match d s0 elt' &&
+   shvec_match s sdenote_desc sdenote_desc_conc_pat elt_match s1 rest')%bool) =
+ true
+).
+Derive Inversion exprinv with (forall d ct mt envd, expr COMPT (hdlr_term ct mt) envd (Desc COMPT d)) Sort Set.
+unfold hdlr_term.
+Open Scope type_scope.
+pose (fun (NB_MSG : nat)
+   (PAYD : (fix vec (n : nat) : Type :=
+              match n with
+              | 0 => unit
+              | S n' =>
+                  (sigT
+                     (fix svec (n0 : nat) : Set :=
+                        match n0 with
+                        | 0 => unit
+                        | S n'0 => desc * svec n'0
+                        end) * vec n')%type
+              end) NB_MSG) (COMPT : Set) (COMPS : COMPT -> compd)
+   (KSTD : sigT
+             (fix svec (n : nat) : Set :=
+                match n with
+                | 0 => unit
+                | S n' => cdesc COMPT * svec n'
+                end)) (d : desc) (ct : COMPT)
+   (mt : (fix fin (n : nat) : Set :=
+            match n with
+            | 0 => False
+            | S n' => option (fin n')
+            end) NB_MSG)
+   (envd : sigT
+             (fix svec (n : nat) : Set :=
+                match n with
+                | 0 => unit
+                | S n' => cdesc COMPT * svec n'
+                end)) =>
+ (let (elt', rest') :=
+      match
+        e in (expr _ _ _ c)
+        return
+          (c = Desc COMPT d ->
+           sdenote_desc_conc_pat d * shvec sdenote_desc_conc_pat s)
+      with
+      | Term d0 H =>
+          fun H0 : d0 = Desc COMPT d =>
+          eq_rec (Desc COMPT d)
+            (fun c : cdesc COMPT =>
+             Reflex.hdlr_term PAYD COMPT COMPS KSTD ct mt envd c ->
+             sdenote_desc_conc_pat d * shvec sdenote_desc_conc_pat s)
+            (fun
+               H1 : Reflex.hdlr_term PAYD COMPT COMPS KSTD ct mt envd
+                      (Desc COMPT d) =>
+             (peval_hdlr_term ct mt H1 (clblr ct),
+             get_conc_pat_conf ct mt envd n s p (clblr ct))) d0
+            (Logic.eq_sym H0) H
+      | UnOp d1 d2 H H0 =>
+          fun H1 : d2 = Desc COMPT d =>
+          eq_rec (Desc COMPT d)
+            (fun c : cdesc COMPT =>
+             unop COMPT d1 c ->
+             expr COMPT (Reflex.hdlr_term PAYD COMPT COMPS KSTD ct mt) envd
+               d1 -> sdenote_desc_conc_pat d * shvec sdenote_desc_conc_pat s)
+            (fun (_ : unop COMPT d1 (Desc COMPT d))
+               (_ : expr COMPT (Reflex.hdlr_term PAYD COMPT COMPS KSTD ct mt)
+                      envd d1) =>
+             (None, get_conc_pat_conf ct mt envd n s p (clblr ct))) d2
+            (Logic.eq_sym H1) H H0
+      | BinOp d1 d2 d3 H H0 H1 =>
+          fun H2 : d3 = Desc COMPT d =>
+          eq_rec (Desc COMPT d)
+            (fun c : cdesc COMPT =>
+             binop COMPT d1 d2 c ->
+             expr COMPT (Reflex.hdlr_term PAYD COMPT COMPS KSTD ct mt) envd
+               d1 ->
+             expr COMPT (Reflex.hdlr_term PAYD COMPT COMPS KSTD ct mt) envd
+               d2 -> sdenote_desc_conc_pat d * shvec sdenote_desc_conc_pat s)
+            (fun (_ : binop COMPT d1 d2 (Desc COMPT d))
+               (_ : expr COMPT (Reflex.hdlr_term PAYD COMPT COMPS KSTD ct mt)
+                      envd d1)
+               (_ : expr COMPT (Reflex.hdlr_term PAYD COMPT COMPS KSTD ct mt)
+                      envd d2) =>
+             (None, get_conc_pat_conf ct mt envd n s p (clblr ct))) d3
+            (Logic.eq_sym H2) H H0 H1
+      end (eq_refl (Desc COMPT d)) in
+  (elt_match d s0 elt' &&
+   shvec_match s sdenote_desc sdenote_desc_conc_pat elt_match s1 rest')%bool) =
+ true).
+inversion e using exprinv.
+Open Scope type_scope.
+pose (fun (NB_MSG : nat)
+   (_ : (fix vec (n : nat) : Type :=
+           match n with
+           | 0 => unit
+           | S n' =>
+               (sigT
+                  (fix svec (n0 : nat) : Set :=
+                     match n0 with
+                     | 0 => unit
+                     | S n'0 => desc * svec n'0
+                     end) * vec n')%type
+           end) NB_MSG) (COMPT : Set) (_ : COMPT -> compd)
+   (_ : sigT
+          (fix svec (n : nat) : Set :=
+             match n with
+             | 0 => unit
+             | S n' => cdesc COMPT * svec n'
+             end)) (d : desc) ct
+   (mt : (fix fin (n : nat) : Set :=
+            match n with
+            | 0 => False
+            | S n' => option (fin n')
+            end) NB_MSG)
+   (envd : sigT
+             (fix svec (n : nat) : Set :=
+                match n with
+                | 0 => unit
+                | S n' => cdesc COMPT * svec n'
+                end)) =>
+ (let (elt', rest') :=
+      match
+        e in (expr _ _ _ c)
+        return
+          (c = Desc _ d ->
+           sdenote_desc_conc_pat d * shvec sdenote_desc_conc_pat s)
+      with
+      | Term d0 H =>
+          fun H0 : d0 = Desc _ d =>
+          eq_rec (Desc COMPT d)
+            (fun c : cdesc COMPT =>
+             Rehdlr_term ct mt envd c ->
+             sdenote_desc_conc_pat d * shvec sdenote_desc_conc_pat s)
+            (fun H1 : hdlr_term ct mt envd (Desc COMPT d) =>
+             (peval_hdlr_term ct mt H1 (clblr ct),
+             get_conc_pat_conf ct mt envd n s p (clblr ct))) d0
+            (Logic.eq_sym H0) H
+      | UnOp d1 d2 H H0 =>
+          fun H1 : d2 = Desc COMPT d =>
+          eq_rec (Desc COMPT d)
+            (fun c : cdesc COMPT =>
+             unop COMPT d1 c ->
+             expr COMPT (hdlr_term ct mt) envd d1 ->
+             sdenote_desc_conc_pat d * shvec sdenote_desc_conc_pat s)
+            (fun (_ : unop COMPT d1 (Desc COMPT d))
+               (_ : expr COMPT (hdlr_term ct mt) envd d1) =>
+             (None, get_conc_pat_conf ct mt envd n s p (clblr ct))) d2
+            (Logic.eq_sym H1) H H0
+      | BinOp d1 d2 d3 H H0 H1 =>
+          fun H2 : d3 = Desc COMPT d =>
+          eq_rec (Desc COMPT d)
+            (fun c : cdesc COMPT =>
+             binop COMPT d1 d2 c ->
+             expr COMPT (hdlr_term ct mt) envd d1 ->
+             expr COMPT (hdlr_term ct mt) envd d2 ->
+             sdenote_desc_conc_pat d * shvec sdenote_desc_conc_pat s)
+            (fun (_ : binop COMPT d1 d2 (Desc COMPT d))
+               (_ : expr COMPT (hdlr_term ct mt) envd d1)
+               (_ : expr COMPT (hdlr_term ct mt) envd d2) =>
+             (None, get_conc_pat_conf ct mt envd n s p (clblr ct))) d3
+            (Logic.eq_sym H2) H H0 H1
+      end (eq_refl (Desc COMPT d)) in
+  (elt_match d s0 elt' &&
+   shvec_match s sdenote_desc sdenote_desc_conc_pat elt_match s1 rest')%bool) =
+ true).
+inversion e using exprinv.
+dependent inversion e with (
+  fun (cd:cdesc COMPT)
+  (e:expr COMPT (Reflex.hdlr_term PAYD COMPT COMPS KSTD ct (tag PAYD m))
+      envd cd) =>
+(let (elt', rest') :=
+        match
+          e in (expr _ _ _ c)
+          return
+            (c = Desc COMPT d ->
+             sdenote_desc_conc_pat d * shvec sdenote_desc_conc_pat s)
+        with
+        | Term d0 H =>
+            fun H0 : d0 = Desc COMPT d =>
+            eq_rec (Desc COMPT d)
+              (fun c : cdesc COMPT =>
+               hdlr_term ct (tag PAYD m) envd c ->
+               sdenote_desc_conc_pat d * shvec sdenote_desc_conc_pat s)
+              (fun H1 : hdlr_term ct (tag PAYD m) envd (Desc COMPT d) =>
+               (peval_hdlr_term ct (tag PAYD m) H1 (clblr ct),
+               get_conc_pat_conf ct (tag PAYD m) envd n s p (clblr ct))) d0
+              (Logic.eq_sym H0) H
+        | UnOp d1 d2 H H0 =>
+            fun H1 : d2 = Desc COMPT d =>
+            eq_rec (Desc COMPT d)
+              (fun c : cdesc COMPT =>
+               unop COMPT d1 c ->
+               expr COMPT (hdlr_term ct (tag PAYD m)) envd d1 ->
+               sdenote_desc_conc_pat d * shvec sdenote_desc_conc_pat s)
+              (fun (_ : unop COMPT d1 (Desc COMPT d))
+                 (_ : expr COMPT (hdlr_term ct (tag PAYD m)) envd d1) =>
+               (None,
+               get_conc_pat_conf ct (tag PAYD m) envd n s p (clblr ct))) d2
+              (Logic.eq_sym H1) H H0
+        | BinOp d1 d2 d3 H H0 H1 =>
+            fun H2 : d3 = Desc COMPT d =>
+            eq_rec (Desc COMPT d)
+              (fun c : cdesc COMPT =>
+               binop COMPT d1 d2 c ->
+               expr COMPT (hdlr_term ct (tag PAYD m)) envd d1 ->
+               expr COMPT (hdlr_term ct (tag PAYD m)) envd d2 ->
+               sdenote_desc_conc_pat d * shvec sdenote_desc_conc_pat s)
+              (fun (_ : binop COMPT d1 d2 (Desc COMPT d))
+                 (_ : expr COMPT (hdlr_term ct (tag PAYD m)) envd d1)
+                 (_ : expr COMPT (hdlr_term ct (tag PAYD m)) envd d2) =>
+               (None,
+               get_conc_pat_conf ct (tag PAYD m) envd n s p (clblr ct))) d3
+              (Logic.eq_sym H2) H H0 H1
+        end (eq_refl cd) in
+    (elt_match d s0 elt' &&
+     shvec_match s sdenote_desc sdenote_desc_conc_pat elt_match s1 rest')%bool) =
+   true).
+
+    shvec_match (n:=S n) (projT2 (existT vdesc' (S n) (d, s))) sdenote_desc
+     sdenote_desc_conc_pat elt_match (s0, s1)
+     (get_conc_pat_conf ct (tag PAYD m) envd
+        (projT1 (existT vdesc' (S n) (d, s)))
+        (projT2 (existT vdesc' (S n) (d, s))) (Some e, p) 
+        (clblr ct)) = true).
+
+
+        auto.
+      generalize s0. rewrite H.
+dependent inversion e with (
+  fun (cd:cdesc COMPT)
+(e:expr COMPT (Reflex.hdlr_term PAYD COMPT COMPS KSTD ct (tag PAYD m))
+        envd cd) =>
+forall s2 : sdenote_desc d,
+   (let (elt', rest') :=
+        match
+          e in (expr _ _ _ c)
+          return
+            (c = cd ->
+             sdenote_desc_conc_pat d * shvec sdenote_desc_conc_pat s)
+        with
+        | Term d0 H =>
+            fun H0 : _ =>
+            eq_rec (Desc COMPT d)
+              (fun c : cdesc COMPT =>
+               hdlr_term ct (tag PAYD m) envd c ->
+               sdenote_desc_conc_pat d * shvec sdenote_desc_conc_pat s)
+              (fun H1 : hdlr_term ct (tag PAYD m) envd (Desc COMPT d) =>
+               (peval_hdlr_term ct (tag PAYD m) H1 (clblr ct),
+               get_conc_pat_conf ct (tag PAYD m) envd n s p (clblr ct))) d0
+              (Logic.eq_sym H0) H
+        | UnOp d1 d2 H H0 =>
+            fun H1 : d2 = Desc COMPT d =>
+            eq_rec (Desc COMPT d)
+              (fun c : cdesc COMPT =>
+               unop COMPT d1 c ->
+               expr COMPT (hdlr_term ct (tag PAYD m)) envd d1 ->
+               sdenote_desc_conc_pat d * shvec sdenote_desc_conc_pat s)
+              (fun (_ : unop COMPT d1 (Desc COMPT d))
+                 (_ : expr COMPT (hdlr_term ct (tag PAYD m)) envd d1) =>
+               (None,
+               get_conc_pat_conf ct (tag PAYD m) envd n s p (clblr ct))) d2
+              (Logic.eq_sym H1) H H0
+        | BinOp d1 d2 d3 H H0 H1 =>
+            fun H2 : d3 = Desc COMPT d =>
+            eq_rec (Desc COMPT d)
+              (fun c : cdesc COMPT =>
+               binop COMPT d1 d2 c ->
+               expr COMPT (hdlr_term ct (tag PAYD m)) envd d1 ->
+               expr COMPT (hdlr_term ct (tag PAYD m)) envd d2 ->
+               sdenote_desc_conc_pat d * shvec sdenote_desc_conc_pat s)
+              (fun (_ : binop COMPT d1 d2 (Desc COMPT d))
+                 (_ : expr COMPT (hdlr_term ct (tag PAYD m)) envd d1)
+                 (_ : expr COMPT (hdlr_term ct (tag PAYD m)) envd d2) =>
+               (None,
+               get_conc_pat_conf ct (tag PAYD m) envd n s p (clblr ct))) d3
+              (Logic.eq_sym H2) H H0 H1
+        end (eq_refl _) in
+    (elt_match d s2 elt' &&
+     shvec_match s sdenote_desc sdenote_desc_conc_pat elt_match s1 rest')%bool) =
+   true
+).
+
+destruct e.
+refine (
+  let elt' :=
+    fst (match
+    e in (expr _ _ _ c)
+    return
+    (c = Desc COMPT d ->
+      sdenote_desc_conc_pat d * shvec sdenote_desc_conc_pat s)
+    with
+    | Term _ _ => _
+    | _ => fun _ => (None, _)
+    end (Logic.eq_refl _)) in
+  _). admit. admit. admit.
+  (elt_match d s0 elt' &&
+    shvec_match s sdenote_desc sdenote_desc_conc_pat elt_match s1 rest')%bool =
+  true).
+
+dependent inversion e.
+        dependent inversion e with (
+fun (d:desc)
+(e:expr COMPT (Reflex.hdlr_term PAYD COMPT COMPS KSTD ct (tag PAYD m))
+        envd (Desc COMPT d))
+=>
+(let (elt', rest') :=
+        match
+          e in (expr _ _ _ c)
+          return
+            (c = Desc COMPT d ->
+             sdenote_desc_conc_pat d * shvec sdenote_desc_conc_pat s)
+        with
+        | Term d0 H =>
+            fun H0 : d0 = Desc COMPT d =>
+            eq_rec (Desc COMPT d)
+              (fun c : cdesc COMPT =>
+               hdlr_term ct (tag PAYD m) envd c ->
+               sdenote_desc_conc_pat d * shvec sdenote_desc_conc_pat s)
+              (fun H1 : hdlr_term ct (tag PAYD m) envd (Desc COMPT d) =>
+               match
+                 H1 in (Reflex.hdlr_term _ _ _ _ _ _ _ c)
+                 return
+                   (c = Desc COMPT d ->
+                    sdenote_desc_conc_pat d * shvec sdenote_desc_conc_pat s)
+               with
+               | Base d1 H2 =>
+                   fun H3 : d1 = Desc COMPT d =>
+                   eq_rec (Desc COMPT d)
+                     (fun c : cdesc COMPT =>
+                      Reflex.base_term COMPT envd c ->
+                      sdenote_desc_conc_pat d * shvec sdenote_desc_conc_pat s)
+                     (fun _ : Reflex.base_term COMPT envd (Desc COMPT d) =>
+                      (None,
+                      get_conc_pat_conf ct (tag PAYD m) envd n s p (clblr ct)))
+                     d1 (Logic.eq_sym H3) H2
+               | CComp =>
+                   fun H2 : Comp COMPT ct = Desc COMPT d =>
+                   False_rec
+                     (sdenote_desc_conc_pat d * shvec sdenote_desc_conc_pat s)
+                     (eq_ind (Comp COMPT ct)
+                        (fun e0 : cdesc COMPT =>
+                         match e0 with
+                         | Desc _ => False
+                         | Comp _ => True
+                         end) I (Desc COMPT d) H2)
+               | CConf ct'0 i H2 =>
+                   fun
+                     H3 : Desc COMPT
+                            (svec_ith
+                               (projT2 (comp_conf_desc COMPT COMPS ct'0)) i) =
+                          Desc COMPT d =>
+                   eq_rec
+                     (svec_ith (projT2 (comp_conf_desc COMPT COMPS ct'0)) i)
+                     (fun d1 : desc =>
+                      Reflex.hdlr_term PAYD COMPT COMPS KSTD ct 
+                        (tag PAYD m) envd (Comp COMPT ct'0) ->
+                      sdenote_desc_conc_pat d1 *
+                      shvec sdenote_desc_conc_pat s)
+                     (fun
+                        H4 : Reflex.hdlr_term PAYD COMPT COMPS KSTD ct
+                               (tag PAYD m) envd (Comp COMPT ct'0) =>
+                      match
+                        H4 in (Reflex.hdlr_term _ _ _ _ _ _ _ c)
+                        return
+                          (c = Comp COMPT ct'0 ->
+                           sdenote_desc_conc_pat
+                             (svec_ith
+                                (projT2 (comp_conf_desc COMPT COMPS ct'0)) i) *
+                           shvec sdenote_desc_conc_pat s)
+                      with
+                      | Base d1 H5 =>
+                          fun H6 : d1 = Comp COMPT ct'0 =>
+                          eq_rec (Comp COMPT ct'0)
+                            (fun c : cdesc COMPT =>
+                             Reflex.base_term COMPT envd c ->
+                             sdenote_desc_conc_pat
+                               (svec_ith
+                                  (projT2 (comp_conf_desc COMPT COMPS ct'0))
+                                  i) * shvec sdenote_desc_conc_pat s)
+                            (fun
+                               _ : Reflex.base_term COMPT envd
+                                     (Comp COMPT ct'0) =>
+                             (None,
+                             get_conc_pat_conf ct (tag PAYD m) envd n s p
+                               (clblr ct))) d1 (Logic.eq_sym H6) H5
+                      | CComp =>
+                          fun H5 : Comp COMPT ct = Comp COMPT ct'0 =>
+                          eq_rec ct
+                            (fun ct'1 : COMPT =>
+                             forall
+                               i0 : fin
+                                      (projT1
+                                         (comp_conf_desc COMPT COMPS ct'1)),
+                             Reflex.hdlr_term PAYD COMPT COMPS KSTD ct
+                               (tag PAYD m) envd (Comp COMPT ct'1) ->
+                             svec_ith
+                               (projT2 (comp_conf_desc COMPT COMPS ct'1)) i0 =
+                             d ->
+                             sdenote_desc_conc_pat
+                               (svec_ith
+                                  (projT2 (comp_conf_desc COMPT COMPS ct'1))
+                                  i0) * shvec sdenote_desc_conc_pat s)
+                            (fun
+                               (i0 : fin
+                                       (projT1
+                                          (comp_conf_desc COMPT COMPS ct)))
+                               (_ : Reflex.hdlr_term PAYD COMPT COMPS KSTD ct
+                                      (tag PAYD m) envd 
+                                      (Comp COMPT ct))
+                               (_ : svec_ith
+                                      (projT2 (comp_conf_desc COMPT COMPS ct))
+                                      i0 = d) =>
+                             (shvec_ith sdenote_desc_conc_pat
+                                (projT2 (compd_conf (COMPS ct))) 
+                                (clblr ct) i0,
+                             get_conc_pat_conf ct (tag PAYD m) envd n s p
+                               (clblr ct))) ct'0
+                            (f_equal
+                               (fun e0 : cdesc COMPT =>
+                                match e0 with
+                                | Desc _ => ct
+                                | Comp c => c
+                                end) H5) i H4
+                            (f_equal
+                               (fun e0 : cdesc COMPT =>
+                                match e0 with
+                                | Desc d1 => d1
+                                | Comp _ =>
+                                    (fix svec_ith (n0 : nat) :
+                                       svec desc n0 -> fin n0 -> desc :=
+                                       match
+                                         n0 as n1
+                                         return
+                                           (svec desc n1 -> fin n1 -> desc)
+                                       with
+                                       | 0 =>
+                                           fun (_ : unit) (idx : False) =>
+                                           match idx return desc with
+                                           end
+                                       | S n' =>
+                                           fun (v : desc * svec desc n')
+                                             (idx : option (fin n')) =>
+                                           match idx with
+                                           | Some idx' =>
+                                               svec_ith n' (snd v) idx'
+                                           | None => fst v
+                                           end
+                                       end)
+                                      (projT1
+                                         (comp_conf_desc COMPT COMPS ct'0))
+                                      (projT2
+                                         (comp_conf_desc COMPT COMPS ct'0)) i
+                                end) H3)
+                      | CConf ct'1 i0 H5 =>
+                          fun
+                            H6 : Desc COMPT
+                                   (svec_ith
+                                      (projT2
+                                         (comp_conf_desc COMPT COMPS ct'1))
+                                      i0) = Comp COMPT ct'0 =>
+                          False_rec
+                            (Reflex.hdlr_term PAYD COMPT COMPS KSTD ct
+                               (tag PAYD m) envd (Comp COMPT ct'1) ->
+                             sdenote_desc_conc_pat
+                               (svec_ith
+                                  (projT2 (comp_conf_desc COMPT COMPS ct'0))
+                                  i) * shvec sdenote_desc_conc_pat s)
+                            (eq_ind
+                               (Desc COMPT
+                                  (svec_ith
+                                     (projT2
+                                        (comp_conf_desc COMPT COMPS ct'1)) i0))
+                               (fun e0 : cdesc COMPT =>
+                                match e0 with
+                                | Desc _ => True
+                                | Comp _ => False
+                                end) I (Comp COMPT ct'0) H6) H5
+                      | MVar i0 =>
+                          fun
+                            H5 : Desc COMPT
+                                   (svec_ith
+                                      (projT2 (lkup_tag PAYD (tag PAYD m)))
+                                      i0) = Comp COMPT ct'0 =>
+                          False_rec
+                            (sdenote_desc_conc_pat
+                               (svec_ith
+                                  (projT2 (comp_conf_desc COMPT COMPS ct'0))
+                                  i) * shvec sdenote_desc_conc_pat s)
+                            (eq_ind
+                               (Desc COMPT
+                                  (svec_ith
+                                     (projT2 (lkup_tag PAYD (tag PAYD m))) i0))
+                               (fun e0 : cdesc COMPT =>
+                                match e0 with
+                                | Desc _ => True
+                                | Comp _ => False
+                                end) I (Comp COMPT ct'0) H5)
+                      | StVar i0 =>
+                          fun _ : svec_ith (projT2 KSTD) i0 = Comp COMPT ct'0 =>
+                          (None,
+                          get_conc_pat_conf ct (tag PAYD m) envd n s p
+                            (clblr ct))
+                      end (eq_refl (Comp COMPT ct'0))) d
+                     (f_equal
+                        (fun e0 : cdesc COMPT =>
+                         match e0 with
+                         | Desc d1 => d1
+                         | Comp _ =>
+                             (fix svec_ith (n0 : nat) :
+                                svec desc n0 -> fin n0 -> desc :=
+                                match
+                                  n0 as n1
+                                  return (svec desc n1 -> fin n1 -> desc)
+                                with
+                                | 0 =>
+                                    fun (_ : unit) (idx : False) =>
+                                    match idx return desc with
+                                    end
+                                | S n' =>
+                                    fun (v : desc * svec desc n')
+                                      (idx : option (fin n')) =>
+                                    match idx with
+                                    | Some idx' => svec_ith n' (snd v) idx'
+                                    | None => fst v
+                                    end
+                                end)
+                               (projT1 (comp_conf_desc COMPT COMPS ct'0))
+                               (projT2 (comp_conf_desc COMPT COMPS ct'0)) i
+                         end) H3) H2
+               | MVar i =>
+                   fun
+                     H2 : Desc COMPT
+                            (svec_ith (projT2 (lkup_tag PAYD (tag PAYD m))) i) =
+                          Desc COMPT d =>
+                   eq_rec (svec_ith (projT2 (lkup_tag PAYD (tag PAYD m))) i)
+                     (fun d1 : desc =>
+                      (sdenote_desc_conc_pat d1 *
+                       shvec sdenote_desc_conc_pat s)%type)
+                     (None,
+                     get_conc_pat_conf ct (tag PAYD m) envd n s p (clblr ct))
+                     d
+                     (f_equal
+                        (fun e0 : cdesc COMPT =>
+                         match e0 with
+                         | Desc d1 => d1
+                         | Comp _ =>
+                             (fix svec_ith (n0 : nat) :
+                                svec desc n0 -> fin n0 -> desc :=
+                                match
+                                  n0 as n1
+                                  return (svec desc n1 -> fin n1 -> desc)
+                                with
+                                | 0 =>
+                                    fun (_ : unit) (idx : False) =>
+                                    match idx return desc with
+                                    end
+                                | S n' =>
+                                    fun (v : desc * svec desc n')
+                                      (idx : option (fin n')) =>
+                                    match idx with
+                                    | Some idx' => svec_ith n' (snd v) idx'
+                                    | None => fst v
+                                    end
+                                end) (projT1 (lkup_tag PAYD (tag PAYD m)))
+                               (projT2 (lkup_tag PAYD (tag PAYD m))) i
+                         end) H2)
+               | StVar i =>
+                   fun _ : svec_ith (projT2 KSTD) i = Desc COMPT d =>
+                   (None,
+                   get_conc_pat_conf ct (tag PAYD m) envd n s p (clblr ct))
+               end (eq_refl (Desc COMPT d))) d0 (Logic.eq_sym H0) H
+        | UnOp d1 d2 H H0 =>
+            fun H1 : d2 = Desc COMPT d =>
+            eq_rec (Desc COMPT d)
+              (fun c : cdesc COMPT =>
+               unop COMPT d1 c ->
+               expr COMPT (hdlr_term ct (tag PAYD m)) envd d1 ->
+               sdenote_desc_conc_pat d * shvec sdenote_desc_conc_pat s)
+              (fun (_ : unop COMPT d1 (Desc COMPT d))
+                 (_ : expr COMPT (hdlr_term ct (tag PAYD m)) envd d1) =>
+               (None,
+               get_conc_pat_conf ct (tag PAYD m) envd n s p (clblr ct))) d2
+              (Logic.eq_sym H1) H H0
+        | BinOp d1 d2 d3 H H0 H1 =>
+            fun H2 : d3 = Desc COMPT d =>
+            eq_rec (Desc COMPT d)
+              (fun c : cdesc COMPT =>
+               binop COMPT d1 d2 c ->
+               expr COMPT (hdlr_term ct (tag PAYD m)) envd d1 ->
+               expr COMPT (hdlr_term ct (tag PAYD m)) envd d2 ->
+               sdenote_desc_conc_pat d * shvec sdenote_desc_conc_pat s)
+              (fun (_ : binop COMPT d1 d2 (Desc COMPT d))
+                 (_ : expr COMPT (hdlr_term ct (tag PAYD m)) envd d1)
+                 (_ : expr COMPT (hdlr_term ct (tag PAYD m)) envd d2) =>
+               (None,
+               get_conc_pat_conf ct (tag PAYD m) envd n s p (clblr ct))) d3
+              (Logic.eq_sym H2) H H0 H1
+        end (eq_refl (Desc COMPT d)) in
+    (elt_match d s0 elt' &&
+     shvec_match s sdenote_desc sdenote_desc_conc_pat elt_match s1 rest')%bool) =
+   true).
+
+Variable ct : COMPT.
+Variable  comp_fd : fd.
+Variable  cfg : sdenote_vdesc (comp_conf_desc COMPT COMPS ct).
+Variable  m : msg PAYD.
+Variable  envd : vcdesc COMPT.
+Variable  ct' : COMPT.
+Variable  comp_fd0 : fd.
+Variable  n : nat.
+Variable  d : desc.
+Variable  s : (fix svec (n : nat) : Set :=
+         match n with
+         | 0 => unit
+         | S n' => (desc * svec n')%type
+         end) n.
+Variable  s0 : sdenote_desc d.
+Variable  s1 : (fix shvec (n : nat) : svec desc n -> Set :=
+          match n as n0 return (svec desc n0 -> Set) with
+          | 0 => fun _ : unit => unit
+          | S n' =>
+              fun v : desc * svec desc n' =>
+              let (t, v') := v in (sdenote_desc t * shvec n' v')%type
+          end) n s.
+Variable  e : expr COMPT (Reflex.hdlr_term PAYD COMPT COMPS KSTD ct (tag PAYD m))
+        envd (Desc COMPT d).
+Variable  p : (fix payload_oexpr' (envd : vcdesc COMPT) (n : nat) 
+                          (pd : vdesc' n) {struct n} : 
+       Type :=
+         match n as _n return (vdesc' _n -> Type) with
+         | 0 => fun _ : unit => unit
+         | S n' =>
+             fun pd0 : desc * vdesc' n' =>
+             let (d, pd') := pd0 in
+             (option
+                (expr COMPT
+                   (Reflex.hdlr_term PAYD COMPT COMPS KSTD ct (tag PAYD m))
+                   envd (Desc COMPT d)) * payload_oexpr' envd n' pd')%type
+         end pd) envd n s.
+Variable  clblr : forall ct : COMPT,
+          shvec sdenote_desc_conc_pat
+            (projT2 (comp_conf_desc COMPT COMPS ct)).
+Variable env : sdenote_vcdesc COMPT COMPS envd.
+Variable st : sdenote_vcdesc COMPT COMPS KSTD.
+Definition stupid :=
+fun (c : cdesc COMPT)
+   (e : expr COMPT (Reflex.hdlr_term PAYD COMPT COMPS KSTD ct (tag PAYD m))
+          envd c) =>
+ (let (elt', rest') :=
+      match
+        e in (expr _ _ _ c0)
+        return
+          (c0 = c -> sdenote_desc_conc_pat d * shvec sdenote_desc_conc_pat s)
+      with
+      | Term d H =>
+          fun H0 : d = c =>
+          eq_rec c
+            (fun c0 : cdesc COMPT =>
+             hdlr_term ct (tag PAYD m) envd c0 ->
+             sdenote_desc_conc_pat d * shvec sdenote_desc_conc_pat s)
+            (fun H1 : hdlr_term ct (tag PAYD m) envd c =>
+             match
+               H1 in (Reflex.hdlr_term _ _ _ _ _ _ _ c0)
+               return
+                 (c0 = c ->
+                  sdenote_desc_conc_pat d * shvec sdenote_desc_conc_pat s)
+             with
+             | Base d0 H2 =>
+                 fun H3 : d0 = c =>
+                 eq_rec c
+                   (fun c0 : cdesc COMPT =>
+                    Reflex.base_term COMPT envd c0 ->
+                    sdenote_desc_conc_pat d * shvec sdenote_desc_conc_pat s)
+                   (fun _ : Reflex.base_term COMPT envd c =>
+                    (None,
+                    get_conc_pat_conf ct (tag PAYD m) envd n s p (clblr ct)))
+                   d0 (Logic.eq_sym H3) H2
+             | CComp =>
+                 fun H2 : Comp COMPT ct = c =>
+                 False_rec
+                   (sdenote_desc_conc_pat d * shvec sdenote_desc_conc_pat s)
+                   (eq_ind (Comp COMPT ct)
+                      (fun e0 : cdesc COMPT =>
+                       match e0 with
+                       | Desc _ => False
+                       | Comp _ => True
+                       end) I c H2)
+             | CConf ct' i H2 =>
+                 fun
+                   H3 : Desc COMPT
+                          (svec_ith (projT2 (comp_conf_desc COMPT COMPS ct'))
+                             i) = c =>
+                 eq_rec
+                   (svec_ith (projT2 (comp_conf_desc COMPT COMPS ct')) i)
+                   (fun d0 : desc =>
+                    Reflex.hdlr_term PAYD COMPT COMPS KSTD ct 
+                      (tag PAYD m) envd (Comp COMPT ct') ->
+                    sdenote_desc_conc_pat d0 * shvec sdenote_desc_conc_pat s)
+                   (fun
+                      H4 : Reflex.hdlr_term PAYD COMPT COMPS KSTD ct
+                             (tag PAYD m) envd (Comp COMPT ct') =>
+                    match
+                      H4 in (Reflex.hdlr_term _ _ _ _ _ _ _ c0)
+                      return
+                        (c0 = Comp COMPT ct' ->
+                         sdenote_desc_conc_pat
+                           (svec_ith
+                              (projT2 (comp_conf_desc COMPT COMPS ct')) i) *
+                         shvec sdenote_desc_conc_pat s)
+                    with
+                    | Base d0 H5 =>
+                        fun H6 : d0 = Comp COMPT ct' =>
+                        eq_rec (Comp COMPT ct')
+                          (fun c0 : cdesc COMPT =>
+                           Reflex.base_term COMPT envd c0 ->
+                           sdenote_desc_conc_pat
+                             (svec_ith
+                                (projT2 (comp_conf_desc COMPT COMPS ct')) i) *
+                           shvec sdenote_desc_conc_pat s)
+                          (fun
+                             _ : Reflex.base_term COMPT envd (Comp COMPT ct') =>
+                           (None,
+                           get_conc_pat_conf ct (tag PAYD m) envd n s p
+                             (clblr ct))) d0 (Logic.eq_sym H6) H5
+                    | CComp =>
+                        fun H5 : Comp COMPT ct = Comp COMPT ct' =>
+                        eq_rec ct
+                          (fun ct'0 : COMPT =>
+                           forall
+                             i0 : fin
+                                    (projT1 (comp_conf_desc COMPT COMPS ct'0)),
+                           Reflex.hdlr_term PAYD COMPT COMPS KSTD ct
+                             (tag PAYD m) envd (Comp COMPT ct'0) ->
+                           svec_ith
+                             (projT2 (comp_conf_desc COMPT COMPS ct'0)) i0 =
+                           d ->
+                           sdenote_desc_conc_pat
+                             (svec_ith
+                                (projT2 (comp_conf_desc COMPT COMPS ct'0)) i0) *
+                           shvec sdenote_desc_conc_pat s)
+                          (fun
+                             (i0 : fin
+                                     (projT1 (comp_conf_desc COMPT COMPS ct)))
+                             (_ : Reflex.hdlr_term PAYD COMPT COMPS KSTD ct
+                                    (tag PAYD m) envd 
+                                    (Comp COMPT ct))
+                             (_ : svec_ith
+                                    (projT2 (comp_conf_desc COMPT COMPS ct))
+                                    i0 = d) =>
+                           (shvec_ith sdenote_desc_conc_pat
+                              (projT2 (compd_conf (COMPS ct))) 
+                              (clblr ct) i0,
+                           get_conc_pat_conf ct (tag PAYD m) envd n s p
+                             (clblr ct))) ct'
+                          (f_equal
+                             (fun e0 : cdesc COMPT =>
+                              match e0 with
+                              | Desc _ => ct
+                              | Comp c0 => c0
+                              end) H5) i H4
+                          (f_equal
+                             (fun e0 : cdesc COMPT =>
+                              match e0 with
+                              | Desc d0 => d0
+                              | Comp _ =>
+                                  (fix svec_ith (n : nat) :
+                                     svec desc n -> fin n -> desc :=
+                                     match
+                                       n as n0
+                                       return
+                                         (svec desc n0 -> fin n0 -> desc)
+                                     with
+                                     | 0 =>
+                                         fun (_ : unit) (idx : False) =>
+                                         match idx return desc with
+                                         end
+                                     | S n' =>
+                                         fun (v : desc * svec desc n')
+                                           (idx : option (fin n')) =>
+                                         match idx with
+                                         | Some idx' =>
+                                             svec_ith n' (snd v) idx'
+                                         | None => fst v
+                                         end
+                                     end)
+                                    (projT1 (comp_conf_desc COMPT COMPS ct'))
+                                    (projT2 (comp_conf_desc COMPT COMPS ct'))
+                                    i
+                              end) H3)
+                    | CConf ct'0 i0 H5 =>
+                        fun
+                          H6 : Desc COMPT
+                                 (svec_ith
+                                    (projT2 (comp_conf_desc COMPT COMPS ct'0))
+                                    i0) = Comp COMPT ct' =>
+                        False_rec
+                          (Reflex.hdlr_term PAYD COMPT COMPS KSTD ct
+                             (tag PAYD m) envd (Comp COMPT ct'0) ->
+                           sdenote_desc_conc_pat
+                             (svec_ith
+                                (projT2 (comp_conf_desc COMPT COMPS ct')) i) *
+                           shvec sdenote_desc_conc_pat s)
+                          (eq_ind
+                             (Desc COMPT
+                                (svec_ith
+                                   (projT2 (comp_conf_desc COMPT COMPS ct'0))
+                                   i0))
+                             (fun e0 : cdesc COMPT =>
+                              match e0 with
+                              | Desc _ => True
+                              | Comp _ => False
+                              end) I (Comp COMPT ct') H6) H5
+                    | MVar i0 =>
+                        fun
+                          H5 : Desc COMPT
+                                 (svec_ith
+                                    (projT2 (lkup_tag PAYD (tag PAYD m))) i0) =
+                               Comp COMPT ct' =>
+                        False_rec
+                          (sdenote_desc_conc_pat
+                             (svec_ith
+                                (projT2 (comp_conf_desc COMPT COMPS ct')) i) *
+                           shvec sdenote_desc_conc_pat s)
+                          (eq_ind
+                             (Desc COMPT
+                                (svec_ith
+                                   (projT2 (lkup_tag PAYD (tag PAYD m))) i0))
+                             (fun e0 : cdesc COMPT =>
+                              match e0 with
+                              | Desc _ => True
+                              | Comp _ => False
+                              end) I (Comp COMPT ct') H5)
+                    | StVar i0 =>
+                        fun _ : svec_ith (projT2 KSTD) i0 = Comp COMPT ct' =>
+                        (None,
+                        get_conc_pat_conf ct (tag PAYD m) envd n s p
+                          (clblr ct))
+                    end (eq_refl (Comp COMPT ct'))) d
+                   (f_equal
+                      (fun e0 : cdesc COMPT =>
+                       match e0 with
+                       | Desc d0 => d0
+                       | Comp _ =>
+                           (fix svec_ith (n : nat) :
+                              svec desc n -> fin n -> desc :=
+                              match
+                                n as n0
+                                return (svec desc n0 -> fin n0 -> desc)
+                              with
+                              | 0 =>
+                                  fun (_ : unit) (idx : False) =>
+                                  match idx return desc with
+                                  end
+                              | S n' =>
+                                  fun (v : desc * svec desc n')
+                                    (idx : option (fin n')) =>
+                                  match idx with
+                                  | Some idx' => svec_ith n' (snd v) idx'
+                                  | None => fst v
+                                  end
+                              end) (projT1 (comp_conf_desc COMPT COMPS ct'))
+                             (projT2 (comp_conf_desc COMPT COMPS ct')) i
+                       end) H3) H2
+             | MVar i =>
+                 fun
+                   H2 : Desc COMPT
+                          (svec_ith (projT2 (lkup_tag PAYD (tag PAYD m))) i) =
+                        c =>
+                 eq_rec (svec_ith (projT2 (lkup_tag PAYD (tag PAYD m))) i)
+                   (fun d0 : desc =>
+                    (sdenote_desc_conc_pat d0 * shvec sdenote_desc_conc_pat s)%type)
+                   (None,
+                   get_conc_pat_conf ct (tag PAYD m) envd n s p (clblr ct)) d
+                   (f_equal
+                      (fun e0 : cdesc COMPT =>
+                       match e0 with
+                       | Desc d0 => d0
+                       | Comp _ =>
+                           (fix svec_ith (n : nat) :
+                              svec desc n -> fin n -> desc :=
+                              match
+                                n as n0
+                                return (svec desc n0 -> fin n0 -> desc)
+                              with
+                              | 0 =>
+                                  fun (_ : unit) (idx : False) =>
+                                  match idx return desc with
+                                  end
+                              | S n' =>
+                                  fun (v : desc * svec desc n')
+                                    (idx : option (fin n')) =>
+                                  match idx with
+                                  | Some idx' => svec_ith n' (snd v) idx'
+                                  | None => fst v
+                                  end
+                              end) (projT1 (lkup_tag PAYD (tag PAYD m)))
+                             (projT2 (lkup_tag PAYD (tag PAYD m))) i
+                       end) H2)
+             | StVar i =>
+                 fun _ : svec_ith (projT2 KSTD) i = c =>
+                 (None,
+                 get_conc_pat_conf ct (tag PAYD m) envd n s p (clblr ct))
+             end (eq_refl c)) d (Logic.eq_sym H0) H
+      | UnOp d1 d2 H H0 =>
+          fun H1 : d2 = c =>
+          eq_rec c
+            (fun c0 : cdesc COMPT =>
+             unop COMPT d1 c0 ->
+             expr COMPT (hdlr_term ct (tag PAYD m)) envd d1 ->
+             sdenote_desc_conc_pat d * shvec sdenote_desc_conc_pat s)
+            (fun (_ : unop COMPT d1 c)
+               (_ : expr COMPT (hdlr_term ct (tag PAYD m)) envd d1) =>
+             (None, get_conc_pat_conf ct (tag PAYD m) envd n s p (clblr ct)))
+            d2 (Logic.eq_sym H1) H H0
+      | BinOp d1 d2 d3 H H0 H1 =>
+          fun H2 : d3 = c =>
+          eq_rec c
+            (fun c0 : cdesc COMPT =>
+             binop COMPT d1 d2 c0 ->
+             expr COMPT (hdlr_term ct (tag PAYD m)) envd d1 ->
+             expr COMPT (hdlr_term ct (tag PAYD m)) envd d2 ->
+             sdenote_desc_conc_pat d * shvec sdenote_desc_conc_pat s)
+            (fun (_ : binop COMPT d1 d2 c)
+               (_ : expr COMPT (hdlr_term ct (tag PAYD m)) envd d1)
+               (_ : expr COMPT (hdlr_term ct (tag PAYD m)) envd d2) =>
+             (None, get_conc_pat_conf ct (tag PAYD m) envd n s p (clblr ct)))
+            d3 (Logic.eq_sym H2) H H0 H1
+      end (eq_refl c) in
+  (elt_match d s0 elt' &&
+   shvec_match s sdenote_desc sdenote_desc_conc_pat elt_match s1 rest')%bool) =
+ true.
+Definition blah :=
+fun (c : cdesc COMPT)
+   (e : expr COMPT (Reflex.hdlr_term PAYD COMPT COMPS KSTD ct (tag PAYD m))
+          envd c) =>
+ (if if (elt_match d s0
+           (eval_oexpr COMPT COMPS
+              (Reflex.hdlr_term PAYD COMPT COMPS KSTD ct (CTAG PAYD m))
+              (fun (d : cdesc COMPT) (envd : vcdesc COMPT)
+                 (e0 : sdenote_vcdesc COMPT COMPS envd)
+                 (t : Reflex.hdlr_term PAYD COMPT COMPS KSTD ct 
+                        (CTAG PAYD m) envd d) =>
+               eval_hdlr_term PAYD COMPT COMPS KSTD
+                 {| comp_type := ct; comp_fd := comp_fd; comp_conf := cfg |}
+                 m st t e0) env (Some e)) &&
+         shvec_match s sdenote_desc sdenote_desc_conc_pat elt_match s1
+           (eval_payload_oexpr' COMPT COMPS
+              (Reflex.hdlr_term PAYD COMPT COMPS KSTD ct (CTAG PAYD m))
+              (fun (d : cdesc COMPT) (envd : vcdesc COMPT)
+                 (e0 : sdenote_vcdesc COMPT COMPS envd)
+                 (t : Reflex.hdlr_term PAYD COMPT COMPS KSTD ct 
+                        (CTAG PAYD m) envd d) =>
+               eval_hdlr_term PAYD COMPT COMPS KSTD
+                 {| comp_type := ct; comp_fd := comp_fd; comp_conf := cfg |}
+                 m st t e0) envd env n s p))%bool
+     then Some (eq_refl ct')
+     else None
+  then true
+  else false) = true ->
+ (let (elt', rest') :=
+      match
+        e in (expr _ _ _ c0)
+        return
+          (c0 = c -> sdenote_desc_conc_pat d * shvec sdenote_desc_conc_pat s)
+      with
+      | Term d H =>
+          fun H0 : d = c =>
+          eq_rec c
+            (fun c0 : cdesc COMPT =>
+             hdlr_term ct (tag PAYD m) envd c0 ->
+             sdenote_desc_conc_pat d * shvec sdenote_desc_conc_pat s)
+            (fun H1 : hdlr_term ct (tag PAYD m) envd c =>
+             match
+               H1 in (Reflex.hdlr_term _ _ _ _ _ _ _ c0)
+               return
+                 (c0 = c ->
+                  sdenote_desc_conc_pat d * shvec sdenote_desc_conc_pat s)
+             with
+             | Base d0 H2 =>
+                 fun H3 : d0 = c =>
+                 eq_rec c
+                   (fun c0 : cdesc COMPT =>
+                    Reflex.base_term COMPT envd c0 ->
+                    sdenote_desc_conc_pat d * shvec sdenote_desc_conc_pat s)
+                   (fun _ : Reflex.base_term COMPT envd c =>
+                    (None,
+                    get_conc_pat_conf ct (tag PAYD m) envd n s p (clblr ct)))
+                   d0 (Logic.eq_sym H3) H2
+             | CComp =>
+                 fun H2 : Comp COMPT ct = c =>
+                 False_rec
+                   (sdenote_desc_conc_pat d * shvec sdenote_desc_conc_pat s)
+                   (eq_ind (Comp COMPT ct)
+                      (fun e0 : cdesc COMPT =>
+                       match e0 with
+                       | Desc _ => False
+                       | Comp _ => True
+                       end) I c H2)
+             | CConf ct' i H2 =>
+                 fun
+                   H3 : Desc COMPT
+                          (svec_ith (projT2 (comp_conf_desc COMPT COMPS ct'))
+                             i) = c =>
+                 eq_rec
+                   (svec_ith (projT2 (comp_conf_desc COMPT COMPS ct')) i)
+                   (fun d0 : desc =>
+                    Reflex.hdlr_term PAYD COMPT COMPS KSTD ct 
+                      (tag PAYD m) envd (Comp COMPT ct') ->
+                    sdenote_desc_conc_pat d0 * shvec sdenote_desc_conc_pat s)
+                   (fun
+                      H4 : Reflex.hdlr_term PAYD COMPT COMPS KSTD ct
+                             (tag PAYD m) envd (Comp COMPT ct') =>
+                    match
+                      H4 in (Reflex.hdlr_term _ _ _ _ _ _ _ c0)
+                      return
+                        (c0 = Comp COMPT ct' ->
+                         sdenote_desc_conc_pat
+                           (svec_ith
+                              (projT2 (comp_conf_desc COMPT COMPS ct')) i) *
+                         shvec sdenote_desc_conc_pat s)
+                    with
+                    | Base d0 H5 =>
+                        fun H6 : d0 = Comp COMPT ct' =>
+                        eq_rec (Comp COMPT ct')
+                          (fun c0 : cdesc COMPT =>
+                           Reflex.base_term COMPT envd c0 ->
+                           sdenote_desc_conc_pat
+                             (svec_ith
+                                (projT2 (comp_conf_desc COMPT COMPS ct')) i) *
+                           shvec sdenote_desc_conc_pat s)
+                          (fun
+                             _ : Reflex.base_term COMPT envd (Comp COMPT ct') =>
+                           (None,
+                           get_conc_pat_conf ct (tag PAYD m) envd n s p
+                             (clblr ct))) d0 (Logic.eq_sym H6) H5
+                    | CComp =>
+                        fun H5 : Comp COMPT ct = Comp COMPT ct' =>
+                        eq_rec ct
+                          (fun ct'0 : COMPT =>
+                           forall
+                             i0 : fin
+                                    (projT1 (comp_conf_desc COMPT COMPS ct'0)),
+                           Reflex.hdlr_term PAYD COMPT COMPS KSTD ct
+                             (tag PAYD m) envd (Comp COMPT ct'0) ->
+                           svec_ith
+                             (projT2 (comp_conf_desc COMPT COMPS ct'0)) i0 =
+                           d ->
+                           sdenote_desc_conc_pat
+                             (svec_ith
+                                (projT2 (comp_conf_desc COMPT COMPS ct'0)) i0) *
+                           shvec sdenote_desc_conc_pat s)
+                          (fun
+                             (i0 : fin
+                                     (projT1 (comp_conf_desc COMPT COMPS ct)))
+                             (_ : Reflex.hdlr_term PAYD COMPT COMPS KSTD ct
+                                    (tag PAYD m) envd 
+                                    (Comp COMPT ct))
+                             (_ : svec_ith
+                                    (projT2 (comp_conf_desc COMPT COMPS ct))
+                                    i0 = d) =>
+                           (shvec_ith sdenote_desc_conc_pat
+                              (projT2 (compd_conf (COMPS ct))) 
+                              (clblr ct) i0,
+                           get_conc_pat_conf ct (tag PAYD m) envd n s p
+                             (clblr ct))) ct'
+                          (f_equal
+                             (fun e0 : cdesc COMPT =>
+                              match e0 with
+                              | Desc _ => ct
+                              | Comp c0 => c0
+                              end) H5) i H4
+                          (f_equal
+                             (fun e0 : cdesc COMPT =>
+                              match e0 with
+                              | Desc d0 => d0
+                              | Comp _ =>
+                                  (fix svec_ith (n : nat) :
+                                     svec desc n -> fin n -> desc :=
+                                     match
+                                       n as n0
+                                       return
+                                         (svec desc n0 -> fin n0 -> desc)
+                                     with
+                                     | 0 =>
+                                         fun (_ : unit) (idx : False) =>
+                                         match idx return desc with
+                                         end
+                                     | S n' =>
+                                         fun (v : desc * svec desc n')
+                                           (idx : option (fin n')) =>
+                                         match idx with
+                                         | Some idx' =>
+                                             svec_ith n' (snd v) idx'
+                                         | None => fst v
+                                         end
+                                     end)
+                                    (projT1 (comp_conf_desc COMPT COMPS ct'))
+                                    (projT2 (comp_conf_desc COMPT COMPS ct'))
+                                    i
+                              end) H3)
+                    | CConf ct'0 i0 H5 =>
+                        fun
+                          H6 : Desc COMPT
+                                 (svec_ith
+                                    (projT2 (comp_conf_desc COMPT COMPS ct'0))
+                                    i0) = Comp COMPT ct' =>
+                        False_rec
+                          (Reflex.hdlr_term PAYD COMPT COMPS KSTD ct
+                             (tag PAYD m) envd (Comp COMPT ct'0) ->
+                           sdenote_desc_conc_pat
+                             (svec_ith
+                                (projT2 (comp_conf_desc COMPT COMPS ct')) i) *
+                           shvec sdenote_desc_conc_pat s)
+                          (eq_ind
+                             (Desc COMPT
+                                (svec_ith
+                                   (projT2 (comp_conf_desc COMPT COMPS ct'0))
+                                   i0))
+                             (fun e0 : cdesc COMPT =>
+                              match e0 with
+                              | Desc _ => True
+                              | Comp _ => False
+                              end) I (Comp COMPT ct') H6) H5
+                    | MVar i0 =>
+                        fun
+                          H5 : Desc COMPT
+                                 (svec_ith
+                                    (projT2 (lkup_tag PAYD (tag PAYD m))) i0) =
+                               Comp COMPT ct' =>
+                        False_rec
+                          (sdenote_desc_conc_pat
+                             (svec_ith
+                                (projT2 (comp_conf_desc COMPT COMPS ct')) i) *
+                           shvec sdenote_desc_conc_pat s)
+                          (eq_ind
+                             (Desc COMPT
+                                (svec_ith
+                                   (projT2 (lkup_tag PAYD (tag PAYD m))) i0))
+                             (fun e0 : cdesc COMPT =>
+                              match e0 with
+                              | Desc _ => True
+                              | Comp _ => False
+                              end) I (Comp COMPT ct') H5)
+                    | StVar i0 =>
+                        fun _ : svec_ith (projT2 KSTD) i0 = Comp COMPT ct' =>
+                        (None,
+                        get_conc_pat_conf ct (tag PAYD m) envd n s p
+                          (clblr ct))
+                    end (eq_refl (Comp COMPT ct'))) d
+                   (f_equal
+                      (fun e0 : cdesc COMPT =>
+                       match e0 with
+                       | Desc d0 => d0
+                       | Comp _ =>
+                           (fix svec_ith (n : nat) :
+                              svec desc n -> fin n -> desc :=
+                              match
+                                n as n0
+                                return (svec desc n0 -> fin n0 -> desc)
+                              with
+                              | 0 =>
+                                  fun (_ : unit) (idx : False) =>
+                                  match idx return desc with
+                                  end
+                              | S n' =>
+                                  fun (v : desc * svec desc n')
+                                    (idx : option (fin n')) =>
+                                  match idx with
+                                  | Some idx' => svec_ith n' (snd v) idx'
+                                  | None => fst v
+                                  end
+                              end) (projT1 (comp_conf_desc COMPT COMPS ct'))
+                             (projT2 (comp_conf_desc COMPT COMPS ct')) i
+                       end) H3) H2
+             | MVar i =>
+                 fun
+                   H2 : Desc COMPT
+                          (svec_ith (projT2 (lkup_tag PAYD (tag PAYD m))) i) =
+                        c =>
+                 eq_rec (svec_ith (projT2 (lkup_tag PAYD (tag PAYD m))) i)
+                   (fun d0 : desc =>
+                    (sdenote_desc_conc_pat d0 * shvec sdenote_desc_conc_pat s)%type)
+                   (None,
+                   get_conc_pat_conf ct (tag PAYD m) envd n s p (clblr ct)) d
+                   (f_equal
+                      (fun e0 : cdesc COMPT =>
+                       match e0 with
+                       | Desc d0 => d0
+                       | Comp _ =>
+                           (fix svec_ith (n : nat) :
+                              svec desc n -> fin n -> desc :=
+                              match
+                                n as n0
+                                return (svec desc n0 -> fin n0 -> desc)
+                              with
+                              | 0 =>
+                                  fun (_ : unit) (idx : False) =>
+                                  match idx return desc with
+                                  end
+                              | S n' =>
+                                  fun (v : desc * svec desc n')
+                                    (idx : option (fin n')) =>
+                                  match idx with
+                                  | Some idx' => svec_ith n' (snd v) idx'
+                                  | None => fst v
+                                  end
+                              end) (projT1 (lkup_tag PAYD (tag PAYD m)))
+                             (projT2 (lkup_tag PAYD (tag PAYD m))) i
+                       end) H2)
+             | StVar i =>
+                 fun _ : svec_ith (projT2 KSTD) i = c =>
+                 (None,
+                 get_conc_pat_conf ct (tag PAYD m) envd n s p (clblr ct))
+             end (eq_refl c)) d (Logic.eq_sym H0) H
+      | UnOp d1 d2 H H0 =>
+          fun H1 : d2 = c =>
+          eq_rec c
+            (fun c0 : cdesc COMPT =>
+             unop COMPT d1 c0 ->
+             expr COMPT (hdlr_term ct (tag PAYD m)) envd d1 ->
+             sdenote_desc_conc_pat d * shvec sdenote_desc_conc_pat s)
+            (fun (_ : unop COMPT d1 c)
+               (_ : expr COMPT (hdlr_term ct (tag PAYD m)) envd d1) =>
+             (None, get_conc_pat_conf ct (tag PAYD m) envd n s p (clblr ct)))
+            d2 (Logic.eq_sym H1) H H0
+      | BinOp d1 d2 d3 H H0 H1 =>
+          fun H2 : d3 = c =>
+          eq_rec c
+            (fun c0 : cdesc COMPT =>
+             binop COMPT d1 d2 c0 ->
+             expr COMPT (hdlr_term ct (tag PAYD m)) envd d1 ->
+             expr COMPT (hdlr_term ct (tag PAYD m)) envd d2 ->
+             sdenote_desc_conc_pat d * shvec sdenote_desc_conc_pat s)
+            (fun (_ : binop COMPT d1 d2 c)
+               (_ : expr COMPT (hdlr_term ct (tag PAYD m)) envd d1)
+               (_ : expr COMPT (hdlr_term ct (tag PAYD m)) envd d2) =>
+             (None, get_conc_pat_conf ct (tag PAYD m) envd n s p (clblr ct)))
+            d3 (Logic.eq_sym H2) H H0 H1
+      end (eq_refl c) in
+  (elt_match d s0 elt' &&
+   shvec_match s sdenote_desc sdenote_desc_conc_pat elt_match s1 rest')%bool) =
+ true.
+
+Definition blah :=
+  fun (c : cdesc COMPT)
+   (e : expr COMPT (Reflex.hdlr_term PAYD COMPT COMPS KSTD ct (tag PAYD m))
+          envd c) =>
+ (let (elt', rest') :=
+      match
+        e in (expr _ _ _ c0)
+        return
+          (c0 = c -> sdenote_desc_conc_pat d * shvec sdenote_desc_conc_pat s)
+      with
+      | Term d H =>
+          fun H0 : d = c =>
+          eq_rec c
+            (fun c0 : cdesc COMPT =>
+             hdlr_term ct (tag PAYD m) envd c0 ->
+             sdenote_desc_conc_pat d * shvec sdenote_desc_conc_pat s)
+            (fun H1 : hdlr_term ct (tag PAYD m) envd c =>
+             match
+               H1 in (Reflex.hdlr_term _ _ _ _ _ _ _ c0)
+               return
+                 (c0 = c ->
+                  sdenote_desc_conc_pat d * shvec sdenote_desc_conc_pat s)
+             with
+             | Base d0 H2 =>
+                 fun H3 : d0 = c =>
+                 eq_rec c
+                   (fun c0 : cdesc COMPT =>
+                    Reflex.base_term COMPT envd c0 ->
+                    sdenote_desc_conc_pat d * shvec sdenote_desc_conc_pat s)
+                   (fun _ : Reflex.base_term COMPT envd c =>
+                    (None,
+                    get_conc_pat_conf ct (tag PAYD m) envd n s p (clblr ct)))
+                   d0 (Logic.eq_sym H3) H2
+             | CComp =>
+                 fun H2 : Comp COMPT ct = c =>
+                 False_rec
+                   (sdenote_desc_conc_pat d * shvec sdenote_desc_conc_pat s)
+                   (eq_ind (Comp COMPT ct)
+                      (fun e0 : cdesc COMPT =>
+                       match e0 with
+                       | Desc _ => False
+                       | Comp _ => True
+                       end) I c H2)
+             | CConf ct' i H2 =>
+                 fun
+                   H3 : Desc COMPT
+                          (svec_ith (projT2 (comp_conf_desc COMPT COMPS ct'))
+                             i) = c =>
+                 eq_rec
+                   (svec_ith (projT2 (comp_conf_desc COMPT COMPS ct')) i)
+                   (fun d0 : desc =>
+                    Reflex.hdlr_term PAYD COMPT COMPS KSTD ct 
+                      (tag PAYD m) envd (Comp COMPT ct') ->
+                    sdenote_desc_conc_pat d0 * shvec sdenote_desc_conc_pat s)
+                   (fun
+                      H4 : Reflex.hdlr_term PAYD COMPT COMPS KSTD ct
+                             (tag PAYD m) envd (Comp COMPT ct') =>
+                    match
+                      H4 in (Reflex.hdlr_term _ _ _ _ _ _ _ c0)
+                      return
+                        (c0 = Comp COMPT ct' ->
+                         sdenote_desc_conc_pat
+                           (svec_ith
+                              (projT2 (comp_conf_desc COMPT COMPS ct')) i) *
+                         shvec sdenote_desc_conc_pat s)
+                    with
+                    | Base d0 H5 =>
+                        fun H6 : d0 = Comp COMPT ct' =>
+                        eq_rec (Comp COMPT ct')
+                          (fun c0 : cdesc COMPT =>
+                           Reflex.base_term COMPT envd c0 ->
+                           sdenote_desc_conc_pat
+                             (svec_ith
+                                (projT2 (comp_conf_desc COMPT COMPS ct')) i) *
+                           shvec sdenote_desc_conc_pat s)
+                          (fun
+                             _ : Reflex.base_term COMPT envd (Comp COMPT ct') =>
+                           (None,
+                           get_conc_pat_conf ct (tag PAYD m) envd n s p
+                             (clblr ct))) d0 (Logic.eq_sym H6) H5
+                    | CComp =>
+                        fun H5 : Comp COMPT ct = Comp COMPT ct' =>
+                        eq_rec ct
+                          (fun ct'0 : COMPT =>
+                           forall
+                             i0 : fin
+                                    (projT1 (comp_conf_desc COMPT COMPS ct'0)),
+                           Reflex.hdlr_term PAYD COMPT COMPS KSTD ct
+                             (tag PAYD m) envd (Comp COMPT ct'0) ->
+                           svec_ith
+                             (projT2 (comp_conf_desc COMPT COMPS ct'0)) i0 =
+                           d ->
+                           sdenote_desc_conc_pat
+                             (svec_ith
+                                (projT2 (comp_conf_desc COMPT COMPS ct'0)) i0) *
+                           shvec sdenote_desc_conc_pat s)
+                          (fun
+                             (i0 : fin
+                                     (projT1 (comp_conf_desc COMPT COMPS ct)))
+                             (_ : Reflex.hdlr_term PAYD COMPT COMPS KSTD ct
+                                    (tag PAYD m) envd 
+                                    (Comp COMPT ct))
+                             (_ : svec_ith
+                                    (projT2 (comp_conf_desc COMPT COMPS ct))
+                                    i0 = d) =>
+                           (shvec_ith sdenote_desc_conc_pat
+                              (projT2 (compd_conf (COMPS ct))) 
+                              (clblr ct) i0,
+                           get_conc_pat_conf ct (tag PAYD m) envd n s p
+                             (clblr ct))) ct'
+                          (f_equal
+                             (fun e0 : cdesc COMPT =>
+                              match e0 with
+                              | Desc _ => ct
+                              | Comp c0 => c0
+                              end) H5) i H4
+                          (f_equal
+                             (fun e0 : cdesc COMPT =>
+                              match e0 with
+                              | Desc d0 => d0
+                              | Comp _ =>
+                                  (fix svec_ith (n : nat) :
+                                     svec desc n -> fin n -> desc :=
+                                     match
+                                       n as n0
+                                       return
+                                         (svec desc n0 -> fin n0 -> desc)
+                                     with
+                                     | 0 =>
+                                         fun (_ : unit) (idx : False) =>
+                                         match idx return desc with
+                                         end
+                                     | S n' =>
+                                         fun (v : desc * svec desc n')
+                                           (idx : option (fin n')) =>
+                                         match idx with
+                                         | Some idx' =>
+                                             svec_ith n' (snd v) idx'
+                                         | None => fst v
+                                         end
+                                     end)
+                                    (projT1 (comp_conf_desc COMPT COMPS ct'))
+                                    (projT2 (comp_conf_desc COMPT COMPS ct'))
+                                    i
+                              end) H3)
+                    | CConf ct'0 i0 H5 =>
+                        fun
+                          H6 : Desc COMPT
+                                 (svec_ith
+                                    (projT2 (comp_conf_desc COMPT COMPS ct'0))
+                                    i0) = Comp COMPT ct' =>
+                        False_rec
+                          (Reflex.hdlr_term PAYD COMPT COMPS KSTD ct
+                             (tag PAYD m) envd (Comp COMPT ct'0) ->
+                           sdenote_desc_conc_pat
+                             (svec_ith
+                                (projT2 (comp_conf_desc COMPT COMPS ct')) i) *
+                           shvec sdenote_desc_conc_pat s)
+                          (eq_ind
+                             (Desc COMPT
+                                (svec_ith
+                                   (projT2 (comp_conf_desc COMPT COMPS ct'0))
+                                   i0))
+                             (fun e0 : cdesc COMPT =>
+                              match e0 with
+                              | Desc _ => True
+                              | Comp _ => False
+                              end) I (Comp COMPT ct') H6) H5
+                    | MVar i0 =>
+                        fun
+                          H5 : Desc COMPT
+                                 (svec_ith
+                                    (projT2 (lkup_tag PAYD (tag PAYD m))) i0) =
+                               Comp COMPT ct' =>
+                        False_rec
+                          (sdenote_desc_conc_pat
+                             (svec_ith
+                                (projT2 (comp_conf_desc COMPT COMPS ct')) i) *
+                           shvec sdenote_desc_conc_pat s)
+                          (eq_ind
+                             (Desc COMPT
+                                (svec_ith
+                                   (projT2 (lkup_tag PAYD (tag PAYD m))) i0))
+                             (fun e0 : cdesc COMPT =>
+                              match e0 with
+                              | Desc _ => True
+                              | Comp _ => False
+                              end) I (Comp COMPT ct') H5)
+                    | StVar i0 =>
+                        fun _ : svec_ith (projT2 KSTD) i0 = Comp COMPT ct' =>
+                        (None,
+                        get_conc_pat_conf ct (tag PAYD m) envd n s p
+                          (clblr ct))
+                    end (eq_refl (Comp COMPT ct'))) d
+                   (f_equal
+                      (fun e0 : cdesc COMPT =>
+                       match e0 with
+                       | Desc d0 => d0
+                       | Comp _ =>
+                           (fix svec_ith (n : nat) :
+                              svec desc n -> fin n -> desc :=
+                              match
+                                n as n0
+                                return (svec desc n0 -> fin n0 -> desc)
+                              with
+                              | 0 =>
+                                  fun (_ : unit) (idx : False) =>
+                                  match idx return desc with
+                                  end
+                              | S n' =>
+                                  fun (v : desc * svec desc n')
+                                    (idx : option (fin n')) =>
+                                  match idx with
+                                  | Some idx' => svec_ith n' (snd v) idx'
+                                  | None => fst v
+                                  end
+                              end) (projT1 (comp_conf_desc COMPT COMPS ct'))
+                             (projT2 (comp_conf_desc COMPT COMPS ct')) i
+                       end) H3) H2
+             | MVar i =>
+                 fun
+                   H2 : Desc COMPT
+                          (svec_ith (projT2 (lkup_tag PAYD (tag PAYD m))) i) =
+                        c =>
+                 eq_rec (svec_ith (projT2 (lkup_tag PAYD (tag PAYD m))) i)
+                   (fun d0 : desc =>
+                    (sdenote_desc_conc_pat d0 * shvec sdenote_desc_conc_pat s)%type)
+                   (None,
+                   get_conc_pat_conf ct (tag PAYD m) envd n s p (clblr ct)) d
+                   (f_equal
+                      (fun e0 : cdesc COMPT =>
+                       match e0 with
+                       | Desc d0 => d0
+                       | Comp _ =>
+                           (fix svec_ith (n : nat) :
+                              svec desc n -> fin n -> desc :=
+                              match
+                                n as n0
+                                return (svec desc n0 -> fin n0 -> desc)
+                              with
+                              | 0 =>
+                                  fun (_ : unit) (idx : False) =>
+                                  match idx return desc with
+                                  end
+                              | S n' =>
+                                  fun (v : desc * svec desc n')
+                                    (idx : option (fin n')) =>
+                                  match idx with
+                                  | Some idx' => svec_ith n' (snd v) idx'
+                                  | None => fst v
+                                  end
+                              end) (projT1 (lkup_tag PAYD (tag PAYD m)))
+                             (projT2 (lkup_tag PAYD (tag PAYD m))) i
+                       end) H2)
+             | StVar i =>
+                 fun _ : svec_ith (projT2 KSTD) i = c =>
+                 (None,
+                 get_conc_pat_conf ct (tag PAYD m) envd n s p (clblr ct))
+             end (eq_refl c)) d (Logic.eq_sym H0) H
+      | UnOp d1 d2 H H0 =>
+          fun H1 : d2 = c =>
+          eq_rec c
+            (fun c0 : cdesc COMPT =>
+             unop COMPT d1 c0 ->
+             expr COMPT (hdlr_term ct (tag PAYD m)) envd d1 ->
+             sdenote_desc_conc_pat d * shvec sdenote_desc_conc_pat s)
+            (fun (_ : unop COMPT d1 c)
+               (_ : expr COMPT (hdlr_term ct (tag PAYD m)) envd d1) =>
+             (None, get_conc_pat_conf ct (tag PAYD m) envd n s p (clblr ct)))
+            d2 (Logic.eq_sym H1) H H0
+      | BinOp d1 d2 d3 H H0 H1 =>
+          fun H2 : d3 = c =>
+          eq_rec c
+            (fun c0 : cdesc COMPT =>
+             binop COMPT d1 d2 c0 ->
+             expr COMPT (hdlr_term ct (tag PAYD m)) envd d1 ->
+             expr COMPT (hdlr_term ct (tag PAYD m)) envd d2 ->
+             sdenote_desc_conc_pat d * shvec sdenote_desc_conc_pat s)
+            (fun (_ : binop COMPT d1 d2 c)
+               (_ : expr COMPT (hdlr_term ct (tag PAYD m)) envd d1)
+               (_ : expr COMPT (hdlr_term ct (tag PAYD m)) envd d2) =>
+             (None, get_conc_pat_conf ct (tag PAYD m) envd n s p (clblr ct)))
+            d3 (Logic.eq_sym H2) H H0 H1
+      end (eq_refl c) in
+  (elt_match d s0 elt' &&
+   shvec_match s sdenote_desc sdenote_desc_conc_pat elt_match s1 rest')%bool) =
+ true.
+
+        dependent inversion e.
+        destruct d. simpl in *. destruct e.
+
+    destruct (COMPTDEC comp_type (conc_pat_type COMPT COMPS x)); try discriminate.
+      destruct x. simpl in *. destruct e. unfold lblr_match_comp.
+      apply existsb_exists. exists ({| conc_pat_type := comp_type; conc_pat_conf := conc_pat_conf |}).
+      split; auto. unfold NIExists.match_comp, Reflex.match_comp, match_comp_pf. simpl.
+      destruct (COMPTDEC comp_type comp_type); try intuition. rewrite UIP_refl with (p:=e). auto.
+  destruct (comp_conf_desc COMPT COMPS cpt).
+  destruct (comp_conf_desc COMPT COMPS
+                                           (comp_pat_type COMPT COMPS
+                                              (hdlr_term
+                                                 (comp_type COMPT COMPS c)
+                                                 (tag PAYD m)) envd cp)).
+  destruct (get_candidate_pats clblr (comp_type COMPT COMPS c)) as [? | ?]_eqn.
+    discriminate.
+
+    apply existsb_exists in Hhigh. destruct Hhigh. destruct H.
+    match goal with
+    | [ _ : context [ cp_incl_dec ?cp1 ?cp2 ] |- _ ]
+      => destruct (cp_incl_dec cp1 cp2); try discriminate
+    end. clear H0. unfold cp_incl in *. unfold high_comp_pat.
+    intros c1 Hmatch'. specialize (c0 c1).
+    unfold match_comp, NIExists.match_comp, Reflex.match_comp, match_comp_pf in *.
+    simpl in *. unfold hdlr_term, CT, CTAG in *.
+    destruct (COMPTDEC (comp_type COMPT COMPS c1)
+                    (comp_pat_type COMPT COMPS
+                       (Reflex.hdlr_term PAYD COMPT COMPS KSTD
+                          (comp_type COMPT COMPS c) 
+                          (tag PAYD m)) envd cp)); try discriminate.
+    simpl in *. destruct c1. destruct cp. simpl in *. destruct e.
+    cut (shvec_match (projT2 (comp_conf_desc COMPT COMPS comp_type))
+                  sdenote_desc sdenote_desc_conc_pat elt_match comp_conf
+                  (get_conc_pat_conf (Reflex.comp_type COMPT COMPS c)
+                     (tag PAYD m) envd
+                     (projT1 (comp_conf_desc COMPT COMPS comp_type))
+                     (projT2 (comp_conf_desc COMPT COMPS comp_type))
+                     comp_pat_conf
+                     (merge_all_cfgps (Reflex.comp_type COMPT COMPS c) l s)) = true).
+      intro. rewrite H0 in *. simpl in *.
+      destruct (COMPTDEC comp_type (conc_pat_type COMPT COMPS x)); try discriminate.
+      destruct x. simpl in *. destruct e. unfold lblr_match_comp.
+      apply existsb_exists. exists ({| conc_pat_type := comp_type; conc_pat_conf := conc_pat_conf |}).
+      split; auto. unfold NIExists.match_comp, Reflex.match_comp, match_comp_pf. simpl.
+      destruct (COMPTDEC comp_type comp_type); try intuition. rewrite UIP_refl with (p:=e). auto.
+      clear c0. destruct (comp_conf_desc COMPT COMPS comp_type) as [n cfgd].
+      induction n.
+        auto.
+
+        destruct cfgd. destruct comp_conf. destruct comp_pat_conf. simpl in *.
+        destruct o.
+          destruct d. destruct e.
+    destruct x. simpl in *. destruct (COMPTDEC comp_type conc_pat_type).
+    destruct e. destruct (comp_conf_desc COMPT COMPS comp_type).
+    Check UIP_refl. rewrite UIP_refl with (p:=e) (x:=comp_pat_type COMPT COMPS
+        (Reflex.hdlr_term PAYD COMPT COMPS KSTD (comp_type COMPT COMPS c)
+           (tag PAYD m)) envd cp) in Hmatch'.
+    induction l.
+      simpl in *.
+    
+    destruct ((cp_incl_dec
+               {|
+               conc_pat_type := comp_pat_type COMPT COMPS
+                                  (hdlr_term (comp_type COMPT COMPS c)
+                                     (tag PAYD m)) envd cp;
+               conc_pat_conf := get_conc_pat_conf (comp_type COMPT COMPS c)
+                                  (tag PAYD m) envd
+                                  (projT1
+                                     (comp_conf_desc COMPT COMPS
+                                        (comp_pat_type COMPT COMPS
+                                           (hdlr_term
+                                              (comp_type COMPT COMPS c)
+                                              (tag PAYD m)) envd cp)))
+                                  (projT2
+                                     (comp_conf_desc COMPT COMPS
+                                        (comp_pat_type COMPT COMPS
+                                           (hdlr_term
+                                              (comp_type COMPT COMPS c)
+                                              (tag PAYD m)) envd cp)))
+                                  (comp_pat_conf COMPT COMPS
+                                     (hdlr_term (comp_type COMPT COMPS c)
+                                        (tag PAYD m)) envd cp)
+                                  (merge_all_cfgps 
+                                     (comp_type COMPT COMPS c) l s) |} x))).
+  destruct (hd_error
+    (get_candidate_pats clblr
+      (comp_type COMPT COMPS c))) as [? | ?]_eqn; try discriminate. SearchAbout hd.
+  induction clblr.
+    discriminate.
+
+    unfold high_comp_pat in *. intros c' Hmatch'. simpl in *.
+    apply Bool.orb_prop in Hmatch. unfold is_high_comp_pat in *.
+    simpl in *. destruct Hmatch.
+      admit.
+
+      rewrite IHclblr; auto. rewrite Bool.orb_true_r. auto.
+  destruct cp as [ctp cfgp]. unfold lblr_match_comp in Hmatch.
+  unfold is_high_comp_pat in *. unfold NIExists.match_comp, Reflex.match_comp, match_comp_pf in *.
+  simpl in *. destruct (COMPTDEC (comp_type COMPT COMPS c') ctp); try discriminate.
+  destruct e.
+  induction clblr.
+    discriminate.
+
+    simpl in *.
+
 
 Ltac uninhabit :=
   match goal with
@@ -44,6 +2608,827 @@ Ltac remove_redundant_ktr :=
       H' : Reflex.ktr _ _ _ _ ?s = inhabits ?tr' |- _ ]
     => rewrite H' in H; apply pack_injective in H; subst tr
   end.
+
+Lemma vlblr_shift : forall n (vlblr:fin (S n) -> bool) (f:fin n),
+  vlblr (Some f) = vlblr (shift_fin f).
+(*  vlblr (Some f) = b -> vlblr (shift_fin f) = b.*)
+Proof.
+  intros n vlblr f.
+  induction n.
+    simpl in *. contradiction.
+
+    simpl. destruct f; auto.
+Qed.
+
+Definition states_ok (s1 s2:kstate) clblr vlblr :=
+  let clblr := lblr_match_comp COMPT COMPTDEC COMPS clblr in
+  high_out_eq _ _ _ _ s1 s2 clblr /\
+    vars_eq _ _ _ _ s1 s2 vlblr.
+
+Definition cmd_ok_low c m envd cmd clblr vlblr :=
+  forall env s i,
+    lblr_match_comp COMPT COMPTDEC COMPS clblr c = false ->
+    states_ok s (hdlr_kst _ _ _ _ _ (ve_st c m envd cmd i {|hdlr_env:=env;hdlr_kst:=s|})) clblr vlblr.
+
+Definition cmd_ok_high c m envd cmd clblr vlblr llblr :=
+  forall env1 env2 s1 s2 i,
+    lblr_match_comp COMPT COMPTDEC COMPS clblr c = true ->
+    states_ok s1 s2 clblr vlblr ->
+    locals_eq envd env1 env2 llblr ->
+    states_ok
+      (hdlr_kst _ _ _ _ _ (ve_st c m envd cmd i {|hdlr_env:=env1;hdlr_kst:=s1|}))
+      (hdlr_kst _ _ _ _ _ (ve_st c m envd cmd i {|hdlr_env:=env2;hdlr_kst:=s2|}))
+      clblr vlblr.
+
+Lemma shvec_erase_ith : forall n vlblr
+  (vd:svec (cdesc COMPT) n) v1 v2,
+  shvec_erase (sdenote_cdesc COMPT COMPS) vlblr vd v1 =
+  shvec_erase (sdenote_cdesc COMPT COMPS) vlblr vd v2 <->
+  (forall i, vlblr i = true ->
+    shvec_ith (sdenote_cdesc COMPT COMPS) vd v1 i =
+    shvec_ith (sdenote_cdesc COMPT COMPS) vd v2 i).
+Proof.
+  intros n vlblr vd v1 v2.
+  induction n.
+    split; intros; auto.
+
+    split.
+      intros Heq i Hlblr.
+      destruct vd; destruct i; simpl in *.
+        destruct v1; destruct v2; simpl in *.
+      apply IHn with (vlblr:=fun f => vlblr (shift_fin f));
+        auto. 
+      match goal with
+      | [ _ : context [ if ?e then _ else _ ] |- _ ]
+        => destruct e
+      end; inversion Heq; auto.
+      rewrite <- vlblr_shift; auto.
+
+      rewrite Hlblr in *. inversion Heq. auto.
+
+      intro H. destruct vd. simpl.
+      match goal with
+      |- context [ if ?e then _ else _ ]
+        => destruct e as [? | ?]_eqn
+      end. f_equal. apply (H None Heqb).
+      apply IHn; auto.
+      intros i Hi.
+      rewrite <- vlblr_shift in Hi.
+      apply (H (Some i) Hi).
+
+      f_equal. apply IHn; auto.
+      intros i Hi.
+      rewrite <- vlblr_shift in Hi.
+      apply (H (Some i) Hi).
+Qed.
+
+Lemma hdlr_expr_ok_high_correct : forall c m (envd:vcdesc COMPT) cd
+  (e:expr _ (hdlr_term (CT _ COMPS c) (CTAG PAYD m)) envd cd)
+  clblr vlblr llblr s1 s2 (env1 env2:sdenote_vcdesc _ _ envd),
+  hdlr_expr_ok_high _ _ _ _ e vlblr llblr = true ->
+  states_ok s1 s2 clblr vlblr ->
+  locals_eq envd env1 env2 llblr ->
+  eval_hdlr_expr _ _ _ _ _ _ (kst _ _ _ _ s1) env1 e =
+  eval_hdlr_expr _ _ _ _ _ _ (kst _ _ _ _ s2) env2 e.
+Proof.
+  intros c m envd cd e clblr vlblr llblr s1 s2 env1 env2 Hexpr Hstates Hlocals.
+  induction e; simpl in *.
+    induction t; simpl in *; auto; try discriminate.
+      destruct b; simpl in *; auto; try discriminate.
+      unfold locals_eq in Hlocals. destruct envd as [? envd]. simpl.
+      eapply shvec_erase_ith with (vd:=envd) (i:=i); eauto.
+
+      rewrite IHt; auto.
+
+      destruct Hstates as [Hout Hvars]. unfold vars_eq in Hvars.
+      destruct s1; destruct s2; destruct KSTD; simpl.
+      eapply shvec_erase_ith with (vd:=v) (v1:=kst)
+        (v2:=kst0) (i:=i); eauto.
+
+    rewrite IHe; auto.
+
+    apply andb_prop in Hexpr. destruct Hexpr.
+    rewrite IHe1; auto. rewrite IHe2; auto.
+Qed.
+
+Lemma expr_list_ok_high_correct : forall c m (envd:vcdesc COMPT) cd
+  (es:list (expr _ (hdlr_term (CT _ COMPS c) (CTAG PAYD m)) envd cd))
+  clblr vlblr llblr s1 s2 (env1 env2:sdenote_vcdesc _ _ envd),
+  expr_list_ok_high _ _ _ _ es vlblr llblr = true ->
+  states_ok s1 s2 clblr vlblr ->
+  locals_eq envd env1 env2 llblr ->
+  map (eval_hdlr_expr _ _ _ _ _ _ (kst _ _ _ _ s1) env1) es =
+  map (eval_hdlr_expr _ _ _ _ _ _ (kst _ _ _ _ s2) env2) es.
+Proof.
+  intros c m envd cd es clblr vlblr llblr
+    s1 s2 env1 env2 Hexpr Hstates Hlocals.
+  induction es.
+    auto.
+
+    simpl in *.
+    destruct (hdlr_expr_ok_high (CT COMPT COMPS c) (CTAG PAYD m) envd cd a vlblr
+             llblr) as [? | ?]_eqn; try discriminate.
+    erewrite hdlr_expr_ok_high_correct; eauto.
+    rewrite IHes; auto.
+Qed.
+
+Lemma pl_hdlr_expr_ok_high_correct : forall c m (envd:vcdesc COMPT) vd
+  (e:payload_expr _ (hdlr_term (CT _ COMPS c) (CTAG PAYD m)) envd vd)
+  clblr vlblr llblr s1 s2 (env1 env2:sdenote_vcdesc _ _ envd),
+  pl_expr_ok_high _ _ _ _ (projT2 vd) e vlblr llblr = true ->
+  states_ok s1 s2 clblr vlblr ->
+  locals_eq envd env1 env2 llblr ->
+  eval_hdlr_payload_expr _ _ _ _ _ _ (kst _ _ _ _ s1) _ env1 _ e =
+  eval_hdlr_payload_expr _ _ _ _ _ _ (kst _ _ _ _ s2) _ env2 _ e.
+Proof.
+  intros c m envd vd e clblr vlblr llblr s1 s2 env1 env2 Hexpr Hstates Hlocals.
+  destruct vd as [n vd].
+  induction n.
+    auto.
+
+    destruct vd. destruct e.
+    unfold eval_hdlr_payload_expr, eval_payload_expr, eval_payload_expr' in *.
+    simpl in *. apply andb_prop in Hexpr. destruct Hexpr as [Hfst ?].
+    eapply hdlr_expr_ok_high_correct in Hfst; eauto.
+    unfold eval_hdlr_expr in Hfst. simpl in *. rewrite Hfst.
+    f_equal. apply IHn; auto.
+Qed.
+
+Fixpoint all_cmd_ok_high c m envd
+  cmd clblr vlblr llblr : Prop :=
+  match cmd in Reflex.cmd _ _ _ _ _ _envd return
+    (fin (projT1 _envd) -> bool) -> _
+  with
+  | Reflex.Seq _ cmd1 cmd2 => fun llblr =>
+    all_cmd_ok_high c m _ cmd1 clblr vlblr llblr /\
+    all_cmd_ok_high c m _ cmd2 clblr vlblr
+      (get_llblr _ _ _ cmd1 vlblr llblr)
+  | Reflex.Ite _ e cmd1 cmd2 => fun llblr =>
+    if hdlr_expr_ok_high _ _ _ _ e vlblr llblr
+    then all_cmd_ok_high c m _ cmd1 clblr vlblr llblr /\
+      all_cmd_ok_high c m _ cmd2 clblr vlblr llblr
+    else False
+(*    all_cmd_ok_high c m _ cmd1 clblr vlblr llblr /\
+    all_cmd_ok_high c m _ cmd2 clblr vlblr llblr*)
+  | Reflex.CompLkup _ _ cmd1 cmd2 => fun llblr => False
+(*    all_cmd_ok_high c m _ cmd1 clblr vlblr llblr /\
+    all_cmd_ok_high c m _ cmd2 clblr vlblr llblr*)
+  | _ => fun _ => cmd_ok_high c m envd cmd clblr vlblr llblr
+  end llblr.
+
+Definition cmd_ok_high' c m envd cmd clblr vlblr llblr :=
+  forall env1 env2 s1 s2 i,
+    lblr_match_comp COMPT COMPTDEC COMPS clblr c = true ->
+    states_ok s1 s2 clblr vlblr ->
+    locals_eq envd env1 env2 llblr ->
+    states_ok
+      (hdlr_kst _ _ _ _ _ (ve_st c m envd cmd i {|hdlr_env:=env1;hdlr_kst:=s1|}))
+      (hdlr_kst _ _ _ _ _ (ve_st c m envd cmd i {|hdlr_env:=env2;hdlr_kst:=s2|}))
+      clblr vlblr /\
+    locals_eq envd
+      (hdlr_env _ _ _ _ _ (ve_st c m envd cmd i {|hdlr_env:=env1;hdlr_kst:=s1|}))
+      (hdlr_env _ _ _ _ _ (ve_st c m envd cmd i {|hdlr_env:=env2;hdlr_kst:=s2|}))
+      (get_llblr _ _ _ cmd vlblr llblr).
+
+Lemma cmd_ok_high'_ok : forall c m envd cmd clblr vlblr llblr,
+  cmd_ok_high' c m envd cmd clblr vlblr llblr ->
+  cmd_ok_high c m envd cmd clblr vlblr llblr.
+Proof.
+  unfold cmd_ok_high, cmd_ok_high'. intros.
+  apply H; auto.
+Qed.
+
+Lemma shvec_erase_wklblr : forall n lblr lblr'
+  (vd:svec (cdesc COMPT) n) v1 v2,
+  (forall i, implb (lblr' i) (lblr i) = true) ->
+  shvec_erase (sdenote_cdesc COMPT COMPS) lblr vd v1 =
+  shvec_erase (sdenote_cdesc COMPT COMPS) lblr vd v2 ->
+  shvec_erase (sdenote_cdesc COMPT COMPS) lblr' vd v1 =
+  shvec_erase (sdenote_cdesc COMPT COMPS) lblr' vd v2.
+Proof.
+  intros n lblr lblr' vd v1 v2 Himpl Herase.
+  rewrite shvec_erase_ith. rewrite shvec_erase_ith in Herase.
+  intros i Hlblr. apply Herase. specialize (Himpl i).
+  rewrite Hlblr in Himpl. unfold implb in Himpl. auto.
+Qed.
+
+Lemma all_cmd_ok_high_correct : forall c m envd cmd clblr vlblr llblr,
+  all_cmd_ok_high c m envd cmd clblr vlblr llblr ->
+  cmd_ok_high' c m envd cmd clblr vlblr llblr.
+Proof.
+  intros c m envd cmd clblr vlblr llblr Hall_ok.
+  unfold cmd_ok_high'.
+  induction cmd; simpl in *; auto.
+    intros. destruct Hall_ok as [Hall_ok1 Hall_ok2].
+    match goal with
+    |- context [ states_ok (hdlr_kst _ _ _ _ _
+      (ve_st _ _ _ _ _ ?s1)) (hdlr_kst _ _ _ _ _
+        (ve_st _ _ _ _ _ ?s2)) _ _ ]
+     => destruct s1 as [s1' env1']_eqn; destruct s2 as [s2' env2']_eqn
+    end. apply IHcmd2; auto.
+      apply f_equal with (f:=hdlr_kst _ _ _ _ _)in Heqh.
+      apply f_equal with (f:=hdlr_kst _ _ _ _ _)in Heqh0.
+      simpl in *. subst s1'. subst s2'. destruct i. simpl.
+      specialize (IHcmd1 llblr Hall_ok1 env1 env2 s1 s2 s H H0). apply IHcmd1; auto.
+      apply f_equal with (f:=hdlr_env _ _ _ _ _)in Heqh.
+      apply f_equal with (f:=hdlr_env _ _ _ _ _)in Heqh0.
+      simpl in *. subst env1'. subst env2'. destruct i. simpl.
+      specialize (IHcmd1 llblr Hall_ok1 env1 env2 s1 s2 s H H0). apply IHcmd1; auto.
+
+    intros. destruct (hdlr_expr_ok_high (CT COMPT COMPS c) 
+    (CTAG PAYD m) envd (Desc COMPT num_d) e vlblr llblr) as [? | ?]_eqn.
+    destruct Hall_ok as [Hall_ok1 Hall_ok2].
+      erewrite hdlr_expr_ok_high_correct; eauto.
+      destruct (num_eq
+              (eval_hdlr_expr PAYD COMPT COMPS KSTD c m
+                 (kst PAYD COMPT COMPS KSTD s2) env2 e) FALSE).
+      unfold locals_eq in *.
+      split.
+        eapply IHcmd2; eauto.
+        apply shvec_erase_wklblr with
+          (lblr:=get_llblr (CT COMPT COMPS c) (CTAG PAYD m) envd cmd2 vlblr
+                llblr). intros.
+        destruct (get_llblr (CT COMPT COMPS c) (CTAG PAYD m) envd cmd1 vlblr llblr i0);
+        destruct (get_llblr (CT COMPT COMPS c) (CTAG PAYD m) envd cmd2 vlblr llblr i0);
+          auto.
+        apply IHcmd2; auto.
+
+      unfold locals_eq in *.
+      split.
+        eapply IHcmd1; eauto.
+        apply shvec_erase_wklblr with
+          (lblr:=get_llblr (CT COMPT COMPS c) (CTAG PAYD m) envd cmd1 vlblr
+                llblr). intros.
+        destruct (get_llblr (CT COMPT COMPS c) (CTAG PAYD m) envd cmd2 vlblr llblr i0);
+        destruct (get_llblr (CT COMPT COMPS c) (CTAG PAYD m) envd cmd1 vlblr llblr i0);
+          auto.
+        apply IHcmd1; auto.
+
+      contradiction.
+
+    unfold cmd_ok_high in *. simpl in *. auto.
+
+    intros. split.
+      unfold cmd_ok_high in *. simpl in *. auto.
+
+      unfold locals_eq in *.
+      apply shvec_erase_ith.
+      destruct (pl_expr_ok_high (CT COMPT COMPS c) (CTAG PAYD m) envd
+        (projT1 (comp_conf_desc COMPT COMPS t))
+        (projT2 (comp_conf_desc COMPT COMPS t)) p vlblr llblr) as [? | ?]_eqn.
+        erewrite pl_hdlr_expr_ok_high_correct; eauto.
+        intros i' ?.
+        destruct (fin_eq_dec i i').
+          subst i'. repeat rewrite shvec_ith_replace_cast_ith. auto.
+          repeat rewrite shvec_ith_replace_cast_other; auto. rewrite shvec_erase_ith in H1. auto.
+
+          intros i' ?. destruct (fin_eq_dec i i'); try discriminate; try contradiction.
+          repeat rewrite shvec_ith_replace_cast_other; auto. rewrite shvec_erase_ith in H1.
+          auto.
+
+    intros. split.
+      unfold cmd_ok_high in *. simpl in *. auto.
+    
+      unfold locals_eq in *.
+      apply shvec_erase_ith.
+      intros i' ?.
+      destruct (fin_eq_dec i i').
+        subst i'. repeat rewrite shvec_ith_replace_cast_ith. auto.
+        repeat rewrite shvec_ith_replace_cast_other; auto. rewrite shvec_erase_ith in H1. auto.
+
+    unfold cmd_ok_high in *. simpl in *. auto.
+
+    contradiction.
+Qed.
+
+(*Lemma get_llblr_correct : forall c m envd cmd i clblr vlblr llblr s1 s2,
+  states_ok (hdlr_kst _ _ _ _ _ s1) (hdlr_kst _ _ _ _ _ s2) clblr vlblr ->
+  locals_eq _ (hdlr_env _ _ _ _ _ s1) (hdlr_env _ _ _ _ _ s2) llblr ->
+(*  all_cmd_ok_high c m envd cmd clblr vlblr llblr ->*)
+  locals_eq _
+    (hdlr_env _ _ _ _ _
+      (ve_st c m envd cmd i s1))
+    (hdlr_env _ _ _ _ _
+      (ve_st c m envd cmd i s2))
+    (get_llblr _ _ _ cmd vlblr llblr).
+Proof.
+  intros c m envd cmd i clblr vlblr llblr s1 s2
+    Hstates Hlocals.
+  generalize dependent s1.
+  generalize dependent s2.
+  induction cmd; auto.
+    (*Seq*)
+    intros s2 s1 Hstates Hlocals. simpl in *.
+    destruct Hall_ok as [Hall_ok1 Hall_ok2].
+    eapply IHcmd2; eauto.
+    match goal with
+      |- context [ve_st _ _ _ _ _ ?s]
+        => let s' := fresh "s'" in
+           let env' := fresh "env'" in
+           destruct s as [s' env']
+    end.
+    destruct (ve_st c m envd cmd1 (fst i)
+              {| hdlr_kst := s1; hdlr_env := env1 |}).
+    destruct (ve_st c m envd cmd1 (fst i)
+              {| hdlr_kst := s2; hdlr_env := env2 |})
+      as [s2' env2']_eqn.
+    destruct (ve_st c m envd cmd1 (fst i)
+              {| hdlr_kst := s1; hdlr_env := env1 |})
+      as [s1' env1']_eqn.
+    eapply IHcmd2; eauto.
+    apply f_equal with (f:=hdlr_env _ _ _ _ _) in Heqh.
+    apply f_equal with (f:=hdlr_env _ _ _ _ _) in Heqh0.
+    simpl in *. subst env1'. subst env2'. auto.
+    apply f_equal with (f:=hdlr_kst _ _ _ _ _) in Heqh.
+    apply f_equal with (f:=hdlr_kst _ _ _ _ _) in Heqh0.
+    simpl in *. subst s1'. subst s2'. auto.
+
+    (*Ite*)
+    intros s2 s1 Hlocals; simpl in *.
+    destruct s1; destruct s2. simpl.
+    rewrite hdlr_expr_ok_high_correct with (s2:=hdlr_kst0)
+      (env2:=hdlr_env0) (clblr:=clblr) (vlblr:=vlblr) (llblr:=llblr);
+      auto.
+
+    (*Spawn*)
+    simpl. unfold locals_eq in *.
+    apply shvec_erase_ith.
+    destruct (pl_expr_ok_high (CT COMPT COMPS c) (CTAG PAYD m) envd
+      (projT1 (comp_conf_desc COMPT COMPS t))
+      (projT2 (comp_conf_desc COMPT COMPS t)) p vlblr llblr) as [? | ?]_eqn.
+      erewrite pl_hdlr_expr_ok_high_correct; eauto.
+      intros i' ?.
+      destruct (fin_eq_dec i0 i').
+        subst i'. repeat rewrite shvec_ith_replace_cast_ith. auto.
+        repeat rewrite shvec_ith_replace_cast_other; auto. rewrite shvec_erase_ith in Hlocals. auto.
+
+      intros i' ?. destruct (fin_eq_dec i0 i'); try discriminate; try contradiction.
+      repeat rewrite shvec_ith_replace_cast_other; auto. rewrite shvec_erase_ith in Hlocals.
+      auto.
+    
+    (*Call*)
+    simpl. unfold locals_eq in *.
+    apply shvec_erase_ith.
+    intros i' ?.
+    destruct (fin_eq_dec i0 i').
+      subst i'. repeat rewrite shvec_ith_replace_cast_ith. auto.
+      repeat rewrite shvec_ith_replace_cast_other; auto. rewrite shvec_erase_ith in Hlocals. auto.*)
+
+Lemma stupd_low : forall clblr vlblr c m envd i e,
+  vlblr i = false ->
+  cmd_ok_low c m envd (StUpd _ _ i e) clblr vlblr.
+Proof.
+  intros clblr vlblr c m envd i e Hvar.
+  split.
+    unfold high_out_eq; simpl.
+    intros tr tr' Htr Htr'. unfold NIExists.ktr in *.
+    rewrite Htr in Htr'. apply pack_injective in Htr'.
+    subst tr. auto.
+
+    unfold vars_eq; simpl.
+    generalize (eval_hdlr_expr PAYD COMPT COMPS KSTD c m
+      (kst PAYD COMPT COMPS KSTD s) env e).
+    simpl in *. clear e. intros.
+    destruct s as [cs tr st].
+    destruct KSTD as [n kstd].
+    induction n.
+      auto.
+
+      destruct kstd. simpl in *.
+      destruct i.
+        match goal with
+        |- context [ if ?e then _ else _ ]
+          => destruct e
+        end; simpl in *.
+          f_equal. destruct st. simpl. apply IHn; auto.
+          rewrite <- vlblr_shift; auto.
+
+          f_equal. destruct st. simpl. apply IHn; auto.
+          rewrite <- vlblr_shift; auto.
+
+        unfold fin in *. rewrite Hvar. f_equal.
+Qed.
+
+Lemma stupd_high : forall c m envd i clblr vlblr llblr
+  (e:expr COMPT (hdlr_term (CT _ _ c) (CTAG _ m)) envd _),
+  vlblr i = false \/
+  hdlr_expr_ok_high _ _ _ _ e vlblr llblr = true ->
+  cmd_ok_high c m envd (StUpd (hdlr_term (CT _ _ c) (CTAG _ m)) envd i e) clblr vlblr llblr.
+Proof.
+  intros c m envd i clblr vlblr llblr e H. destruct H as [Hlblr | Hexpr].
+    split.
+      unfold states_ok, high_out_eq in *. simpl. apply H0.
+
+      unfold states_ok, vars_eq in *; simpl.
+      generalize (eval_hdlr_expr PAYD COMPT COMPS KSTD c m
+        (kst PAYD COMPT COMPS KSTD s1) env1 e).
+      generalize (eval_hdlr_expr PAYD COMPT COMPS KSTD c m
+        (kst PAYD COMPT COMPS KSTD s2) env2 e).
+      simpl in *. clear e. intros.
+      destruct s1 as [cs1 tr1 st1].
+      destruct s2 as [cs2 tr2 st2].
+      destruct KSTD as [n kstd].
+      induction n.
+        auto.
+
+        destruct kstd. simpl in *. destruct H0.
+        destruct i.
+        match goal with
+        |- context [ if ?e then _ else _ ]
+          => destruct e
+        end; simpl in *.
+        inversion H2. f_equal. destruct st1. destruct st2.
+        simpl. apply IHn; auto.
+        rewrite <- vlblr_shift; auto.
+        
+        inversion H2. f_equal. destruct st1. destruct st2.
+        simpl. apply IHn; auto.
+        rewrite <- vlblr_shift; auto.
+        
+        unfold fin in *. rewrite Hlblr in *.
+        inversion H2. simpl. f_equal. auto.
+        
+    split.
+
+      unfold states_ok, high_out_eq in *. simpl. apply H0.
+      
+      unfold vars_eq in *; simpl.
+      erewrite hdlr_expr_ok_high_correct
+        with (env1:=env1) (env2:=env2); eauto.
+      generalize (eval_hdlr_expr PAYD COMPT COMPS KSTD c m
+        (kst PAYD COMPT COMPS KSTD s2) env2 e).
+      destruct s1; destruct s2. simpl in *. clear Hexpr e.
+      simpl. destruct H0 as [Hout Hvars]. clear Hout.
+      destruct KSTD as [n kstd]. unfold vars_eq in *.
+      simpl in *. intros.
+      induction n.
+        auto.
+        
+        destruct kstd.
+        destruct i; simpl in *;
+          match goal with
+          |- context [if ?e then _ else _ ]
+            => destruct e
+          end; inversion Hvars; f_equal;
+          apply IHn; auto.
+Qed.
+
+Lemma stupd_high_all : forall c m envd i clblr vlblr llblr
+  (e:expr COMPT (hdlr_term (CT _ _ c) (CTAG _ m)) envd _),
+  vlblr i = false \/
+  hdlr_expr_ok_high _ _ _ _ e vlblr llblr = true ->
+  all_cmd_ok_high c m envd (StUpd (hdlr_term (CT _ _ c) (CTAG _ m)) envd i e) clblr vlblr llblr.
+Proof.
+  apply stupd_high.
+Qed.
+
+Fixpoint match_all_cfg_pat n : forall (vd:svec desc n),
+  shvec sdenote_desc_conc_pat vd :=
+  match n as _n return
+    forall (_vd:svec desc _n), shvec sdenote_desc_conc_pat _vd
+  with
+  | O => fun _ => tt
+  | S n' => fun vd =>
+    match vd with
+    | (vd0, vd') =>
+      (None, match_all_cfg_pat n' vd')
+    end
+  end.
+
+Definition match_all_pat ct :=
+  {| conc_pat_type:=ct
+    ; conc_pat_conf:=match_all_cfg_pat _
+    (projT2 (comp_conf_desc COMPT COMPS ct)) |}.
+
+Lemma match_all_pat_correct : forall ct c,
+  comp_type _ _ c = ct ->
+  match_comp (match_all_pat ct) c = true.
+Proof.
+  intros ct c Hct. unfold match_all_pat.
+  unfold match_comp, Reflex.match_comp, match_comp_pf.
+  destruct (COMPTDEC (comp_type COMPT COMPS c)
+           (conc_pat_type COMPT COMPS
+              {|
+              conc_pat_type := ct;
+              conc_pat_conf := match_all_cfg_pat
+                                 (projT1 (comp_conf_desc COMPT COMPS ct))
+                                 (projT2 (comp_conf_desc COMPT COMPS ct)) |})); try contradiction.
+  simpl in *. subst ct. rewrite UIP_refl with (p:=e).
+  destruct c. simpl in *. destruct (comp_conf_desc COMPT COMPS comp_type) as [n cfg].
+  induction n.
+    auto.
+
+    destruct cfg. destruct comp_conf. simpl in *. apply IHn.
+Qed.
+Require Import Sumbool.
+
+Definition ct_not_in_clblr ct clblr :=
+  forallb (fun cp => negb (projT1 (bool_of_sumbool
+    (COMPTDEC ct (conc_pat_type COMPT COMPS cp))))) clblr = true.
+
+Lemma not_in_clblr : forall ct clblr,
+  ct_not_in_clblr ct clblr ->
+  forall c, comp_type COMPT COMPS c = ct ->
+    lblr_match_comp _ COMPTDEC _ clblr c = false.
+Proof.
+  intros ct clblr Hnot_in c Hct. unfold lblr_match_comp.
+  induction clblr.
+    auto.
+
+    unfold lblr_match_comp in *.
+    unfold ct_not_in_clblr in Hnot_in. simpl in *. apply andb_prop in Hnot_in.
+    destruct Hnot_in. 
+    unfold NIExists.match_comp, Reflex.match_comp, match_comp_pf in *.
+    destruct c. simpl in *. subst comp_type.
+    destruct (COMPTDEC ct (conc_pat_type COMPT COMPS a)); try discriminate.
+    rewrite Bool.orb_false_r. auto.
+Qed.
+  
+Lemma send_low : forall c m envd clblr vlblr ct
+  ce t ple,
+  ct_not_in_clblr ct clblr ->
+  cmd_ok_low c m envd (Send _ envd ct ce t ple) clblr vlblr.
+Proof.
+  intros c m envd clblr vlblr ct ce t ple Hnot_in.
+  unfold cmd_ok_low, states_ok. intros.
+  split.
+    unfold high_out_eq. intros. destruct s as [? [?] ?].
+    simpl in *. repeat uninhabit. simpl. erewrite not_in_clblr; eauto.
+    destruct (eval_hdlr_expr PAYD COMPT COMPS KSTD c m kst env ce). auto.
+
+    unfold vars_eq. simpl. auto.
+Qed.
+
+Lemma send_low_ccomp : forall c m envd clblr vlblr t ple,
+  cmd_ok_low c m envd (Send _ envd _
+    (Term _ _ _ (CComp _ _ _ _ _ _ _)) t ple) clblr vlblr.
+Proof.
+  intros c m envd clblr vlblr t ple.
+  unfold cmd_ok_low, states_ok. intros.
+  split.
+    unfold high_out_eq. intros. destruct s as [? [?] ?].
+    simpl in *. repeat uninhabit. simpl. rewrite H. auto.
+
+    unfold vars_eq. simpl. auto.
+Qed.
+
+Lemma send_high_all : forall c m envd clblr vlblr llblr ct
+  ce t ple,
+  hdlr_expr_ok_high _ _ _ _ ce vlblr llblr = true ->
+  pl_expr_ok_high _ _ _ _ _ ple vlblr llblr = true ->
+  all_cmd_ok_high c m envd (Send _ envd ct ce t ple) clblr vlblr llblr.
+Proof.
+  simpl. unfold cmd_ok_high. unfold states_ok. simpl.
+  intros c m envd clblr vlblr llblr ct ce t ple Hexpr
+    Hpexpr env1 env2 s1 s2 i Hlblr Hstates Hlocals.
+  split.
+    unfold high_out_eq. intros tr tr' Htr Htr'.
+    destruct s1 as [? [ ? ] ?]_eqn. destruct s2 as [? [ ? ] ?]_eqn. simpl in *.
+    repeat uninhabit. simpl. inversion Heqk. inversion Heqk0.
+    apply f_equal with (f:=Reflex.kst _ _ _ _) in Heqk.
+    apply f_equal with (f:=Reflex.kst _ _ _ _) in Heqk0.
+    simpl in *. rewrite <- Heqk. rewrite <- Heqk0.
+    destruct Hstates as [Hout Hvars]. unfold high_out_eq in Hout.
+    erewrite Hout; eauto.
+    erewrite hdlr_expr_ok_high_correct with (s2:=s2) (clblr:=clblr); eauto.
+    erewrite pl_hdlr_expr_ok_high_correct with (s2:=s2) (clblr:=clblr); eauto.
+    subst s1. subst s2. unfold states_ok. auto.
+    subst s1. subst s2. unfold states_ok. auto.
+
+    unfold vars_eq in *. simpl. apply Hstates.
+Qed.
+
+Lemma send_high_all_low_comp : forall c m envd clblr vlblr llblr ct
+  ce t ple,
+  ct_not_in_clblr ct clblr ->
+  all_cmd_ok_high c m envd (Send _ envd ct ce t ple) clblr vlblr llblr.
+Proof.
+  intros c m envd clblr vlblr llblr ct ce t ple Hnot_in.
+  simpl. unfold cmd_ok_high, states_ok. intros.
+  split.
+    unfold high_out_eq in *. intros. destruct s1 as [? [?] ?]; destruct s2 as [? [?] ?].
+    simpl in *. repeat uninhabit. simpl. repeat erewrite not_in_clblr; eauto.
+    destruct H0. auto.
+    destruct (eval_hdlr_expr PAYD COMPT COMPS KSTD c m kst0 env2 ce). auto.
+    destruct (eval_hdlr_expr PAYD COMPT COMPS KSTD c m kst env1 ce). auto.
+
+    unfold vars_eq. simpl. destruct H0. auto.
+Qed.
+
+Lemma call_low : forall c m envd clblr vlblr
+  e es i EQ,
+  cmd_ok_low c m envd (Call _ envd e es i EQ) clblr vlblr.
+Proof.
+  intros c m envd clblr vlblr e es i EQ.
+  simpl. unfold cmd_ok_low. intros.
+  unfold states_ok, high_out_eq, vars_eq in *. simpl.
+  split.
+    intros. destruct s as [? [?] ?].
+    simpl in *. repeat uninhabit. simpl. auto.
+
+    auto.
+Qed.
+
+Lemma call_high_all : forall c m envd clblr vlblr llblr
+  e es i EQ,
+  all_cmd_ok_high c m envd (Call _ envd e es i EQ) clblr vlblr llblr.
+Proof.
+  intros c m envd clblr vlblr llblr e es i EQ.
+  simpl. unfold cmd_ok_high. intros.
+  unfold states_ok, high_out_eq, vars_eq in *. simpl.
+  split.
+    intros. destruct s1 as [? [?] ?]; destruct s2 as [? [?] ?].
+    simpl in *. repeat uninhabit. simpl. destruct H0. erewrite H0; eauto.
+
+    apply H0.
+Qed.
+
+Lemma spawn_high_all : forall c m envd clblr vlblr llblr ct
+  ple i EQ,
+  pl_expr_ok_high _ _ _ _ _ ple vlblr llblr = true ->
+  all_cmd_ok_high c m envd (Spawn _ envd ct ple i EQ) clblr vlblr llblr.
+Proof.
+  simpl. unfold cmd_ok_high. unfold states_ok. simpl.
+  intros c m envd clblr vlblr llblr ct ple i EQ
+    Hpexpr env1 env2 s1 s2 f Hlblr Hstates Hlocals.
+  split.
+    unfold high_out_eq. intros tr tr' Htr Htr'.
+    destruct s1 as [? [ ? ] ?]_eqn. destruct s2 as [? [ ? ] ?]_eqn. simpl in *.
+    repeat uninhabit. simpl. inversion Heqk. inversion Heqk0.
+    apply f_equal with (f:=Reflex.kst _ _ _ _) in Heqk.
+    apply f_equal with (f:=Reflex.kst _ _ _ _) in Heqk0.
+    simpl in *. rewrite <- Heqk. rewrite <- Heqk0.
+    destruct Hstates as [Hout Hvars]. unfold high_out_eq in Hout.
+    erewrite Hout; eauto.
+    erewrite pl_hdlr_expr_ok_high_correct with (s2:=s2) (clblr:=clblr); eauto.
+    subst s1. subst s2. unfold states_ok. auto.
+
+    unfold vars_eq in *. simpl. apply Hstates.
+Qed.
+
+Lemma ite_low : forall c m envd clblr vlblr
+  e cmd1 cmd2,
+  cmd_ok_low c m envd cmd1 clblr vlblr ->
+  cmd_ok_low c m envd cmd2 clblr vlblr ->
+  cmd_ok_low c m envd (Ite _ envd e cmd1 cmd2) clblr vlblr.
+Proof.
+  intros c m envd clblr vlblr e cmd1 cmd2 Hcmd1 Hcmd2.
+  unfold cmd_ok_low in *. intros env s i. simpl.
+  destruct (num_eq
+              (eval_hdlr_expr PAYD COMPT COMPS KSTD c m
+                 (kst PAYD COMPT COMPS KSTD s) env e) FALSE); auto.
+Qed.
+
+Lemma ite_high_all : forall c m envd clblr vlblr llblr
+  e cmd1 cmd2,
+  hdlr_expr_ok_high _ _ _ _ e vlblr llblr = true ->
+  all_cmd_ok_high c m envd cmd1 clblr vlblr llblr ->
+  all_cmd_ok_high c m envd cmd2 clblr vlblr llblr ->
+  all_cmd_ok_high c m envd (Ite _ envd e cmd1 cmd2) clblr vlblr llblr.
+Proof.
+  intros c m envd clblr vlblr llblr e cmd1 cmd2 Hexpr Hcmd1 Hcmd2.
+  simpl. rewrite Hexpr. auto.
+Qed.
+
+Lemma seq_low : forall clblr vlblr c m envd cmd1 cmd2,
+  cmd_ok_low c m envd cmd1 clblr vlblr ->
+  cmd_ok_low c m envd cmd2 clblr vlblr ->
+  cmd_ok_low c m envd (Seq _ _ cmd1 cmd2) clblr vlblr.
+Proof.
+  intros clblr vlblr c m envd cmd1 cmd2 Hcmd1 Hcmd2.
+  split.
+    unfold cmd_ok_low, high_out_eq, ve_st, kstate_run_prog in *. simpl in *.
+    intros. destruct i as [i1 i2]. specialize (Hcmd1 env s i1 H).
+    destruct Hcmd1 as [Hout1 ?].
+    destruct (hdlr_state_run_cmd PAYD COMPT COMPTDEC COMPS KSTD c m envd
+                  {| hdlr_kst := s; hdlr_env := env |} cmd1 i1) as [st env']_eqn.
+    specialize (Hcmd2 env' st i2 H). destruct Hcmd2 as [Hout2 ?].
+    destruct st as [? [tr''] ?]. simpl in *. rewrite Hout1 with (tr':=tr''); auto.
+    apply Hout2 with (tr:=tr'') (tr':=tr'); auto. rewrite <- Heqh. auto.
+
+    unfold cmd_ok_low, vars_eq, ve_st, kstate_run_prog in *. simpl in *.
+    destruct i as [i1 i2].
+    specialize (Hcmd1 env s i1 H). destruct Hcmd1 as [? Hvar1].
+    destruct (hdlr_state_run_cmd PAYD COMPT COMPTDEC COMPS KSTD c m envd
+                  {| hdlr_kst := s; hdlr_env := env |} cmd1 i1) as [st env']_eqn.
+    specialize (Hcmd2 env' st i2 H). destruct Hcmd2 as [? Hvar2].
+    rewrite Hvar1. simpl in *. rewrite Heqh. apply Hvar2.
+Qed.
+
+Lemma seq_high_all : forall c m envd cmd1 cmd2 clblr vlblr llblr,
+  all_cmd_ok_high c m envd cmd1 clblr vlblr llblr ->
+  all_cmd_ok_high c m envd cmd2 clblr vlblr
+    (get_llblr (CT _ _ c) (CTAG _ m) envd cmd1 vlblr llblr) ->
+  all_cmd_ok_high c m envd (Seq _ _ cmd1 cmd2) clblr vlblr llblr.
+Proof.
+  simpl. auto.
+Qed.
+(*  intros c m envd cmd1 cmd2 clblr vlblr llblr Hcmd1 Hcmd2.
+    unfold cmd_ok_high, high_out_eq, ve_st, kstate_run_prog in *. simpl in *.
+    intros. destruct i as [i1 i2]. specialize (Hcmd1 env1 env2 s1 s2 i1 H H0).
+    simpl in *.
+    destruct (hdlr_state_run_cmd PAYD COMPT COMPTDEC COMPS KSTD c m envd
+                  {| hdlr_kst := s1; hdlr_env := env1 |} cmd1 i1) as [s1' env1']_eqn.
+    destruct (hdlr_state_run_cmd PAYD COMPT COMPTDEC COMPS KSTD c m envd
+                  {| hdlr_kst := s2; hdlr_env := env2 |} cmd1 i1) as [s2' env2']_eqn.
+    simpl in *.
+    apply Hcmd2; intuition.
+    apply f_equal with (f:=hdlr_env _ _ _ _ _) in Heqh.
+    apply f_equal with (f:=hdlr_env _ _ _ _ _) in Heqh0.
+    simpl in *. subst env1'. subst env2'.
+    eapply get_llblr_correct; eauto.
+Qed.*)
+
+Lemma high_out_eq_inter_ve_st : forall c m s tr clblr,
+  Reflex.ktr _ _ _ _ s = [tr]%inhabited ->
+  high_out_eq _ _ _ _ s (mk_inter_ve_st PAYD COMPT COMPS KSTD c m s tr) clblr.
+Proof.
+  unfold high_out_eq, mk_inter_ve_st. simpl. intros.
+  remove_redundant_ktr. repeat uninhabit. auto.
+Qed.
+
+Lemma high_out_trans : forall (s1 s2 s3:kstate) clblr,
+  high_out_eq _ _ _ _ s1 s2 clblr ->
+  high_out_eq _ _ _ _ s2 s3 clblr ->
+  high_out_eq _ _ _ _ s1 s3 clblr.
+Proof.
+  intros. unfold high_out_eq in *.
+  intros. destruct s2. destruct ktr0.
+  rewrite <- H0 with (tr:=k) (tr':=tr'); auto.
+Qed.
+
+Lemma high_out_eq_refl : forall (s:kstate) clblr,
+  high_out_eq _ _ _ _ s s clblr.
+Proof.
+  intros. unfold high_out_eq. intros.
+  remove_redundant_ktr. auto.
+Qed.
+
+Lemma vars_eq_refl : forall (s:kstate) vlblr,
+  vars_eq _ _ _ _ s s vlblr.
+Proof.
+  auto.
+Qed.
+
+Lemma high_out_eq_sym : forall (s s':kstate) clblr,
+  high_out_eq _ _ _ _ s s' clblr ->
+  high_out_eq _ _ _ _ s' s clblr.
+Proof.
+  unfold high_out_eq. intros.
+  symmetry. auto.
+Qed.
+
+Lemma vars_eq_sym : forall (s s':kstate) vlblr,
+  vars_eq _ _ _ _ s s' vlblr ->
+  vars_eq _ _ _ _ s' s vlblr.
+Proof.
+  unfold vars_eq. intros. auto.
+Qed.
+
+Lemma vars_eq_inter_ve_st : forall c m s tr clblr,
+  Reflex.ktr _ _ _ _ s = [tr]%inhabited ->
+  vars_eq _ _ _ _ s (mk_inter_ve_st PAYD COMPT COMPS KSTD c m s tr) clblr.
+Proof.
+  auto.
+Qed.
+
+Lemma vars_eq_trans : forall (s1 s2 s3:kstate) clblr,
+  vars_eq _ _ _ _ s1 s2 clblr ->
+  vars_eq _ _ _ _ s2 s3 clblr ->
+  vars_eq _ _ _ _ s1 s3 clblr.
+Proof.
+  intros. unfold vars_eq in *. etransitivity; eauto.
+Qed.
+
+Lemma nop_low : forall clblr vlblr c m envd,
+  cmd_ok_low c m envd (Nop _ _) clblr vlblr.
+Proof.
+  intros clblr vlblr c m envd.
+  unfold cmd_ok_low, states_ok. intros env s.
+  simpl. split.
+    apply high_out_eq_refl.
+    apply vars_eq_refl.
+Qed.
+
+Lemma nop_high : forall clblr vlblr c m envd llblr,
+  cmd_ok_high c m envd (Nop _ _) clblr vlblr llblr.
+Proof.
+  intros clblr vlblr c m envd llblr.
+  unfold cmd_ok_high, states_ok. intros.
+  simpl. auto.
+Qed.
+
+Lemma nop_high_all : forall clblr vlblr c m envd llblr,
+  all_cmd_ok_high c m envd (Nop _ _) clblr vlblr llblr.
+Proof.
+  apply nop_high.
+Qed.
+
+Section WITH_HANDLERS_INIT.
+
+Variable HANDLERS : handlers PAYD COMPT COMPS KSTD.
+Variable INIT : init_prog PAYD COMPT COMPS KSTD IENVD.
+Definition ValidExchange := Reflex.ValidExchange PAYD COMPT COMPTDEC COMPS KSTD HANDLERS.
 
 Lemma prune_nop_1 : forall clblr vlblr c m i s s',
   ValidExchange c m i s s' ->
@@ -60,6 +3445,28 @@ Proof.
       uninhabit. simpl. remove_redundant_ktr. auto.
 
       unfold vars_eq. simpl. auto.
+Qed.
+
+Lemma prune_nop_1' : forall clblr vlblr c m i s tr,
+  projT2 (HANDLERS (tag _ m) (comp_type COMPT COMPS c)) =
+  Nop _ _ ->
+  Reflex.ktr _ _ _ _ s = [tr]%inhabited ->
+  high_out_eq _ _ _ _ s
+    (kstate_run_prog PAYD COMPT COMPTDEC COMPS KSTD c m
+    (projT1 (HANDLERS (tag PAYD m) (comp_type COMPT COMPS c)))
+    (mk_inter_ve_st PAYD COMPT COMPS KSTD c m s tr)
+    (projT2 (HANDLERS (tag PAYD m) (comp_type COMPT COMPS c))) i)
+    clblr /\
+    vars_eq _ _ _ _ s
+      (kstate_run_prog PAYD COMPT COMPTDEC COMPS KSTD c m
+      (projT1 (HANDLERS (tag PAYD m) (comp_type COMPT COMPS c)))
+      (mk_inter_ve_st PAYD COMPT COMPS KSTD c m s tr)
+      (projT2 (HANDLERS (tag PAYD m) (comp_type COMPT COMPS c))) i)
+      vlblr.
+Proof.
+  intros.
+  eapply prune_nop_1; eauto.
+  econstructor; eauto.
 Qed.
 
 Lemma prune_nop_2 : forall clblr vlblr c m i s1 s1' s2 s2',
@@ -80,6 +3487,57 @@ Proof.
 
       unfold vars_eq. simpl. auto.
 Qed.
+
+Lemma prune_nop_2' : forall clblr vlblr c m i s1 s2 tr1 tr2,
+  projT2 (HANDLERS (tag _ m) (comp_type COMPT COMPS c)) =
+  Nop _ _ ->
+  Reflex.ktr _ _ _ _ s1 = [tr1]%inhabited ->
+  Reflex.ktr _ _ _ _ s2 = [tr2]%inhabited ->
+  high_out_eq _ _ _ _ s1 s2 clblr -> vars_eq _ _ _ _ s1 s2 vlblr ->
+  high_out_eq _ _ _ _
+    (kstate_run_prog PAYD COMPT COMPTDEC COMPS KSTD c m
+      (projT1 (HANDLERS (tag PAYD m) (comp_type COMPT COMPS c)))
+      (mk_inter_ve_st PAYD COMPT COMPS KSTD c m s1 tr1)
+      (projT2 (HANDLERS (tag PAYD m) (comp_type COMPT COMPS c))) i)
+      (kstate_run_prog PAYD COMPT COMPTDEC COMPS KSTD c m
+      (projT1 (HANDLERS (tag PAYD m) (comp_type COMPT COMPS c)))
+      (mk_inter_ve_st PAYD COMPT COMPS KSTD c m s2 tr2)
+      (projT2 (HANDLERS (tag PAYD m) (comp_type COMPT COMPS c))) i)
+      clblr /\
+    vars_eq _ _ _ _
+      (kstate_run_prog PAYD COMPT COMPTDEC COMPS KSTD c m
+      (projT1 (HANDLERS (tag PAYD m) (comp_type COMPT COMPS c)))
+      (mk_inter_ve_st PAYD COMPT COMPS KSTD c m s1 tr1)
+      (projT2 (HANDLERS (tag PAYD m) (comp_type COMPT COMPS c))) i)
+      (kstate_run_prog PAYD COMPT COMPTDEC COMPS KSTD c m
+      (projT1 (HANDLERS (tag PAYD m) (comp_type COMPT COMPS c)))
+      (mk_inter_ve_st PAYD COMPT COMPS KSTD c m s2 tr2)
+      (projT2 (HANDLERS (tag PAYD m) (comp_type COMPT COMPS c))) i)
+      vlblr.
+Proof.
+  intros.
+  eapply prune_nop_2; eauto;
+  econstructor; eauto.
+Qed.
+
+Definition low_ok'' clblr vlblr := forall c m,
+  lblr_match_comp COMPT COMPTDEC COMPS clblr c = false ->
+  cmd_ok_low c m (projT1 (HANDLERS (tag PAYD m) (comp_type COMPT COMPS c)))
+    (projT2 (HANDLERS (tag PAYD m) (comp_type COMPT COMPS c))) clblr vlblr.
+
+Definition high_ok'' clblr vlblr :=
+  forall c m,
+    lblr_match_comp COMPT COMPTDEC COMPS clblr c = true ->
+    cmd_ok_high c m (projT1 (HANDLERS (tag PAYD m) (comp_type COMPT COMPS c)))
+    (projT2 (HANDLERS (tag PAYD m) (comp_type COMPT COMPS c)))
+    clblr vlblr (fun _ => true).
+
+Definition high_ok_all clblr vlblr :=
+  forall c m,
+    lblr_match_comp COMPT COMPTDEC COMPS clblr c = true ->
+    all_cmd_ok_high c m (projT1 (HANDLERS (tag PAYD m) (comp_type COMPT COMPS c)))
+    (projT2 (HANDLERS (tag PAYD m) (comp_type COMPT COMPS c)))
+    clblr vlblr (fun _ => true).
 
 (*
 Print high_ok.
@@ -116,5 +3574,50 @@ Proof.
     unfold kstate_run_prog. unfold hdlr_state_run_cmd.
         
 *)
+
+Theorem ni_suf'' : forall clblr vlblr,
+  low_ok'' clblr vlblr ->
+  high_ok'' clblr vlblr ->
+  NI PAYD COMPT COMPTDEC COMPS
+  IENVD KSTD INIT HANDLERS clblr vlblr.
+Proof.
+  intros. apply ni_suf'.
+  unfold low_ok', low_ok'', cmd_ok_low, states_ok, ve_st in *.
+  intros.
+  split.
+    apply high_out_trans with (s2:=mk_inter_ve_st PAYD COMPT COMPS KSTD c m s tr); auto.
+    apply high_out_eq_inter_ve_st; auto.
+    apply H; auto.
+    apply vars_eq_trans with (s2:=mk_inter_ve_st PAYD COMPT COMPS KSTD c m s tr); auto.
+    apply H; auto.
+
+  unfold high_ok', high_ok'', cmd_ok_high, states_ok, ve_st in *.
+  intros. apply H0; auto.
+  split.
+    apply high_out_trans with (s2:=s1). apply high_out_eq_sym.
+    apply high_out_eq_inter_ve_st; auto.
+    apply high_out_eq_sym. apply high_out_trans with (s2:=s2).
+    apply high_out_eq_sym. apply high_out_eq_inter_ve_st; auto.
+    apply high_out_eq_sym; auto.
+
+    apply vars_eq_trans with (s2:=s1). apply vars_eq_sym.
+    apply vars_eq_inter_ve_st; auto.
+    apply vars_eq_sym. apply vars_eq_trans with (s2:=s2).
+    apply vars_eq_sym. apply vars_eq_inter_ve_st; auto.
+    apply vars_eq_sym; auto.
+Qed.
+
+Theorem ni_suf_all : forall clblr vlblr,
+  low_ok'' clblr vlblr ->
+  high_ok_all clblr vlblr ->
+  NI PAYD COMPT COMPTDEC COMPS
+  IENVD KSTD INIT HANDLERS clblr vlblr.
+Proof.
+  intros. apply ni_suf''; auto.
+    unfold high_ok''. intros. apply cmd_ok_high'_ok.
+    apply all_cmd_ok_high_correct; auto.
+Qed.
+
+End WITH_HANDLERS_INIT.
 
 End Prune.
