reflex/coq/bench-enables/Kernel.v
@@ -79,3 +79,27 @@ Definition HANDLERS : handlers PAYD COMPT COMPS KSTD :=
   | _, _ => [[ mk_vcdesc [] : nop ]]
   end.
 Close Scope hdlr.
+<<<<<<< Updated upstream:reflex/coq/bench-enables/Kernel.v
+=======
+
+Require Import PolLang.
+Require Import ActionMatch.
+Require Import List.
+
+Local Opaque str_of_string.
+
+Theorem enable : forall st tr u,
+  Reach PAYD COMPT COMPTDEC COMPS KSTD IENVD INIT HANDLERS st ->
+  ktr _ _ _ _ st = inhabits tr ->
+  Enables PAYD COMPT COMPS COMPTDEC
+          (KORecv PAYD COMPT COMPS None
+                   (Some (Build_opt_msg PAYD
+                                         LoginResT (Some u, tt))))
+          (KOSend PAYD COMPT COMPS None
+                   (Some (Build_opt_msg PAYD
+                                         PrivReq (Some u, tt))))
+          tr.
+Proof.
+  Time crush.
+Qed.
+>>>>>>> Stashed changes:reflex/coq/EnablesTest.v
