reflex/coq/bench-quark/Kernel.v
@@ -43,8 +43,8 @@ Definition PAYD : vvdesc NB_MSG := mk_vvdesc
   ; ("KeyPress",    [str_d])
   ; ("MouseClick",  [str_d; str_d; num_d])
   ; ("Go",          [str_d])
-  ; ("NewTab",      [])
-  ; ("CProcFD", [fd_d])
+  ; ("NewTab",      [str_d])
+  ; ("CKChan",      [fd_d])
   ].
 
 Notation Display     := 0%fin (only parsing).
@@ -58,7 +58,7 @@ Notation KeyPress    := 7%fin (only parsing).
 Notation MouseClick  := 8%fin (only parsing).
 Notation Go          := 9%fin (only parsing).
 Notation NewTab      := 10%fin (only parsing).
-Notation CProcFD     := 11%fin (only parsing).
+Notation CKChan      := 11%fin (only parsing).
 
 Inductive COMPT' : Set := UserInput | Output | Tab | CProc | DomainBar.
 
@@ -79,11 +79,13 @@ Definition COMPS (t : COMPT) : compd :=
   end.
 
 Definition IENVD : vcdesc COMPT := mk_vcdesc
-  [ Comp _ Output; Comp _ Tab; Comp _ UserInput ].
+  [ Comp _ Output; Comp _ Tab; Comp _ UserInput; Comp _ CProc; Desc _ fd_d ].
 
 Notation i_output    := 0%fin (only parsing).
 Notation i_curtab    := 1%fin (only parsing).
 Notation i_userinput := 2%fin (only parsing).
+Notation i_ckproc    := 3%fin (only parsing).
+Notation i_ckchan    := 4%fin (only parsing).
 
 Definition KSTD : vcdesc COMPT := mk_vcdesc
   [ Comp _ Output; Comp _ Tab ].
@@ -114,11 +116,15 @@ Close Scope char_scope.
 Definition INIT : init_prog PAYD COMPT COMPS KSTD IENVD :=
   seq (spawn _ IENVD Output    tt                   i_output    (Logic.eq_refl _)) (
   seq (spawn _ IENVD Tab       (i_slit default_domain, tt) i_curtab    (Logic.eq_refl _)) (
+  seq (spawn _ IENVD CProc     (i_slit default_domain, tt) i_ckproc    (Logic.eq_refl _)) (
+  seq (call _ IENVD (i_slit (str_of_string (test_dir ++ "ckchan.py"))) [] i_ckchan (Logic.eq_refl _)) (
+  seq (send (i_envvar IENVD i_curtab) CKChan (i_envvar IENVD i_ckchan, tt)) (
+  seq (send (i_envvar IENVD i_ckproc) CKChan (i_envvar IENVD i_ckchan, tt)) (
   seq (spawn _ IENVD UserInput tt                   i_userinput (Logic.eq_refl _)) (
   seq (send (i_envvar IENVD i_curtab) Go (i_slit default_url, tt)) (
   seq (stupd _ IENVD v_output (Term _ (base_term _ ) _ (Var _ IENVD i_output))) (
   seq (stupd _ IENVD v_curtab (Term _ (base_term _ ) _ (Var _ IENVD i_curtab))
-  ) nop))))).
+  ) nop))))))))).
 
 Definition cur_tab_dom {t envd} :=
   cconf (envd:=envd) (t:=t) Tab Tab 0%fin (CComp PAYD COMPT COMPS KSTD Tab t envd).
@@ -172,19 +178,6 @@ Definition HANDLERS : handlers PAYD COMPT COMPS KSTD :=
                nop
              )
        ]]
-  | Tab, CProcFD =>
-      let envd := mk_vcdesc [Comp _ CProc] in
-      [[ envd :
-        complkup (envd:=envd) (mk_comp_pat _ _ CProc (Some cur_tab_dom, tt))
-                 (send (ct:=CProc) (term:=mk_vcdesc [Comp _ CProc; Comp _ CProc])
-                   (envd:=hdlr_term SystemFeatures.PAYD
-                   SystemFeatures.COMPT SystemFeatures.COMPS
-                   SystemFeatures.KSTD Tab CProcFD)
-                   (envvar (cc:=Tab) (m:=CProcFD) (mk_vcdesc [Comp _ CProc; Comp _ CProc]) 1%fin)
-                   CProcFD (mvar CProcFD 0%fin, tt))
-                 (seq (spawn _ envd CProc (cur_tab_dom, tt) 0%fin (Logic.eq_refl _)) (
-                      (send (envvar envd 0%fin) CProcFD (mvar CProcFD 0%fin, tt))))
-      ]]
   | UserInput, KeyPress =>
       [[ mk_vcdesc [] :
       seq (send (stvar v_curtab) KeyPress (mvar KeyPress None, tt))
@@ -195,17 +188,177 @@ Definition HANDLERS : handlers PAYD COMPT COMPS KSTD :=
         (mvar MouseClick 0%fin, (mvar MouseClick 1%fin, (mvar MouseClick 2%fin, tt))))
       nop ]]
   | UserInput, NewTab =>
-      let envd := mk_vcdesc [Comp _ Tab] in
+      let envd := mk_vcdesc [Comp _ Tab; Comp _ CProc; Desc _ fd_d] in
       [[ envd :
-         seq (spawn _ envd Tab (slit default_domain, tt) None (Logic.eq_refl _)) (
+         seq (spawn _ envd Tab (dom (mvar NewTab 0%fin), tt) None (Logic.eq_refl _)) (
          seq (stupd _ envd v_curtab (envvar envd None)) (
-         seq (send (stvar v_curtab) Go (slit default_url, tt))
-             nop))
+         seq (call _ envd (slit (str_of_string (test_dir ++ "ckchan.py"))) [] 2%fin (Logic.eq_refl _)) (
+         seq (send (stvar v_curtab) CKChan (envvar envd 2%fin, tt)) (
+         seq nop(*(complkup (envd:=envd) (mk_comp_pat _ _ CProc (Some (dom (mvar NewTab 0%fin)), tt))
+                 (send (ct:=CProc) (term:=mk_vcdesc [Comp _ Tab; Comp _ CProc; Desc _ fd_d; Comp _ CProc])
+                   (envd:=hdlr_term SystemFeatures.PAYD
+                   SystemFeatures.COMPT SystemFeatures.COMPS
+                   SystemFeatures.KSTD UserInput NewTab)
+                   (envvar (cc:=UserInput) (m:=NewTab) (mk_vcdesc [Comp _ Tab; Comp _ CProc; Desc _ fd_d; Comp _ CProc]) 3%fin)
+                   CKChan ((envvar (cc:=UserInput) (m:=NewTab) (mk_vcdesc [Comp _ Tab; Comp _ CProc; Desc _ fd_d; Comp _ CProc]) 2%fin), tt))
+                 (seq (spawn _ envd CProc (dom (mvar NewTab 0%fin), tt) 1%fin (Logic.eq_refl _)) (
+                      (send (envvar envd 1%fin) CKChan (envvar envd 2%fin, tt)))))*) ( 
+         seq (send (stvar v_curtab) Go (mvar NewTab 0%fin, tt))
+             nop)))))
       ]]
   | _, _ =>
     [[ mk_vcdesc [] : nop ]]
   end.
 Close Scope hdlr.
+<<<<<<< Updated upstream:reflex/coq/bench-quark/Kernel.v
+=======
+(*Definition HANDLERS : handlers PAYD COMPT COMPS KSTD :=
+  (fun m cc =>
+     let (ct, cf, cconf) := cc in
+     match ct, tag PAYD m as _tm return
+       @sdenote _ SDenoted_vdesc (lkup_tag PAYD _tm) -> _
+     with
+
+     | Tab, Display => fun pl =>
+       let envd := mk_vcdesc [] in
+       match pl with (disp, _) =>
+       existT
+         (fun d => hdlr_prog PAYD COMPT COMPS KSTD cc m d) envd
+         (fun st0 =>
+            if fd_eq cf (comp_fd (kst_ith st0 v_curtab))
+            then
+              [ fun s => sendall envd _
+                                 (mk_comp_pat
+                                    Tab
+                                    (Some (comp_fd s##v_output%kst))
+                                    (None, tt)
+                                 )
+                                 Display (slit disp, tt)
+              ]
+            else
+              []
+         )
+       end
+
+     | Tab, Navigate => fun pl =>
+       let envd := mk_vcdesc [Comp _ Tab] in
+       match pl with (url, _) =>
+       existT
+         (fun d => hdlr_prog PAYD COMPT COMPS KSTD cc m d) envd
+         (fun st0 =>
+            if fd_eq cf (comp_fd (kst_ith st0 v_curtab))
+            then
+              if str_eq (dom url)
+                        (
+                          shvec_ith (n := (projT1 (compd_conf (COMPS Tab))))
+                            sdenote_desc
+                            (projT2 (compd_conf (COMPS Tab)))
+                            (comp_conf (st0##v_curtab%kst))
+                            None
+                        )
+              then
+                [ fun s => spawn envd _ Tab (dom url, tt) None (Logic.eq_refl _)
+                ; fun s => stupd envd _ v_curtab (envvar envd None)
+                ; fun s => sendall envd _
+                             (mk_comp_pat
+                                Tab
+                                (Some (comp_fd s##v_curtab%kst))
+                                (None, tt)
+                             )
+                             Go (slit url, tt)
+                ]
+              else
+                []
+            else
+              []
+         )
+       end
+
+     | Tab, ReqResource => fun pl =>
+       let envd := mk_vcdesc [] in
+       match pl with (url, _) =>
+       existT
+         (fun d => hdlr_prog PAYD COMPT COMPS KSTD cc m d) envd
+         (
+           nop
+         )
+       end
+
+    end (pay PAYD m)
+  ).
+*)
+
+
+Require Import NIExists.
+
+Open Scope char_scope.
+Definition dom' s :=
+  let url_end := snd (splitAt "." s) in
+  fst (splitAt "/" url_end).
+Close Scope char_scope.
+Print conc_pat.
+
+Definition clblr (d:str) :=
+  [Build_conc_pat COMPT COMPS Tab (Some d, tt);
+   Build_conc_pat COMPT COMPS CProc (Some d, tt);
+   Build_conc_pat COMPT COMPS UserInput tt].
+
+(*  match c
+  with
+  | Build_comp Tab _ cfg =>
+    let cfgd := comp_conf_desc COMPT COMPS Tab in
+    if str_eq (@shvec_ith _ _ (projT1 cfgd) (projT2 cfgd)
+                               cfg None) d
+    then true
+    else false
+  | Build_comp CProc _ cfg =>
+    let cfgd := comp_conf_desc COMPT COMPS Tab in
+    if str_eq (@shvec_ith _ _ (projT1 cfgd) (projT2 cfgd)
+                               cfg None) d
+    then true
+    else false
+  | Build_comp UserInput _ _ => true
+  | _ => false
+  end.
+*)
+
+Definition vlblr (f : fin (projT1 KSTD)) := true.
+
+Local Opaque str_of_string.
+
+Require Import PruneFacts.
+Theorem ni : forall d, NI PAYD COMPT COMPTDEC COMPS
+  IENVD KSTD INIT HANDLERS (clblr d) vlblr.
+Proof.
+  intros; apply ni_suf_all.
+Local Opaque cmd_ok_low.
+    Time unfold low_ok''; intros;
+    destruct_msg'; destruct_comp';
+    try discriminate; simpl;
+      repeat first [apply nop_low
+        | apply seq_low
+        | apply ite_low
+        | apply stupd_low
+        | solve [apply send_low_ccomp]
+        | apply send_low
+        | apply call_low
+        | solve [auto] ].
+
+Local Opaque all_cmd_ok_high.
+    Time unfold high_ok_all; intros;
+    destruct_msg'; destruct_comp';
+    try discriminate; simpl;
+      repeat first [apply nop_high_all
+        | apply seq_high_all
+        | apply ite_high_all
+        | apply stupd_high_all
+        | solve [apply send_high_all_low_comp; auto]
+        | apply send_high_all
+        | apply spawn_high_all
+        | apply call_high_all
+        | solve [auto ] ].
+Qed.
+>>>>>>> Stashed changes:reflex/coq/ReflexQuark.v
 
 End Spec.
 
